infoflow: Arch arch split
Signed-off-by: Ryan Barry <ryan.barry@unsw.edu.au>

proof/infoflow/Arch_IF.thy
@@ -5,828 +5,150 @@
  *)
 
 theory Arch_IF
-imports Retype_IF
+imports ArchRetype_IF
 begin
-
-context begin interpretation Arch . (*FIXME: arch_split*)
 
 abbreviation irq_state_of_state :: "det_state \<Rightarrow> nat" where
   "irq_state_of_state s \<equiv> irq_state (machine_state s)"
 
+
+crunches cap_insert, cap_swap_for_delete
+  for irq_state_of_state[wp]: "\<lambda>s. P (irq_state_of_state s)"
+  (wp: crunch_wps)
+
 lemma do_extended_op_irq_state_of_state[wp]:
-  "\<lbrace>\<lambda>s. P (irq_state_of_state s)\<rbrace> do_extended_op f \<lbrace>\<lambda>_ s. P (irq_state_of_state s)\<rbrace>"
+  "do_extended_op f \<lbrace>\<lambda>s. P (irq_state_of_state s)\<rbrace>"
   by (wpsimp wp: dxo_wp_weak)
 
 lemma no_irq_underlying_memory_update[simp]:
   "no_irq (modify (underlying_memory_update f))"
   by (wpsimp simp: no_irq_def)
 
-crunch irq_state_of_state[wp]: cap_insert "\<lambda>s. P (irq_state_of_state s)"
-  (wp: crunch_wps)
-
-crunch irq_state_of_state[wp]: set_extra_badge "\<lambda>s. P (irq_state_of_state s)"
-  (wp: crunch_wps dmo_wp simp: storeWord_def)
-
-
-lemma transfer_caps_loop_irq_state[wp]:
-  "\<lbrace>\<lambda>s. P (irq_state_of_state s)\<rbrace> transfer_caps_loop a b c d e f \<lbrace>\<lambda>_ s. P (irq_state_of_state s)\<rbrace>"
-  apply(wp transfer_caps_loop_pres)
-  done
-
-crunch irq_state_of_state[wp]: set_mrs "\<lambda>s. P (irq_state_of_state s)"
-  (wp: crunch_wps dmo_wp simp: crunch_simps maskInterrupt_def store_word_offs_def storeWord_def ignore: const_on_failure)
-
-crunch irq_state_of_state[wp]: handle_recv "\<lambda>s. P (irq_state_of_state s)"
-  (wp: crunch_wps dmo_wp simp: crunch_simps maskInterrupt_def store_word_offs_def storeWord_def ignore: const_on_failure)
-
-crunch irq_state_of_state[wp]: handle_reply "\<lambda>s. P (irq_state_of_state s)"
-  (wp: crunch_wps dmo_wp simp: crunch_simps maskInterrupt_def unless_def store_word_offs_def storeWord_def ignore: const_on_failure)
-
-crunch irq_state_of_state[wp]: handle_vm_fault, handle_hypervisor_fault "\<lambda>s. P (irq_state_of_state s)"
-  (wp: crunch_wps dmo_wp simp: crunch_simps maskInterrupt_def unless_def store_word_offs_def storeWord_def ignore: const_on_failure getFAR getDFSR getIFSR simp: getDFSR_def no_irq_getFAR getFAR_def getIFSR_def)
-
-
-lemma irq_state_clearExMonitor[wp]: "\<lbrace> \<lambda>s. P (irq_state s) \<rbrace> clearExMonitor \<lbrace> \<lambda>_ s. P (irq_state s) \<rbrace>"
-  apply (simp add: clearExMonitor_def | wp modify_wp)+
-  done
-
-crunch irq_state_of_state[wp]: schedule "\<lambda>(s::det_state). P (irq_state_of_state s)"
-  (wp: dmo_wp modify_wp crunch_wps hoare_whenE_wp
-       simp: invalidateLocalTLB_ASID_def setHardwareASID_def set_current_pd_def
-             machine_op_lift_def machine_rest_lift_def crunch_simps storeWord_def
-             dsb_def isb_def writeTTBR0_def)
-
-crunch irq_state_of_state[wp]: reply_from_kernel "\<lambda>s. P (irq_state_of_state s)"
-
-
 lemma detype_irq_state_of_state[simp]:
   "irq_state_of_state (detype S s) = irq_state_of_state s"
-  apply(simp add: detype_def)
-  done
-
-text \<open>Not true of invoke_untyped any more.\<close>
-crunch irq_state_of_state[wp]: retype_region,create_cap,delete_objects "\<lambda>s. P (irq_state_of_state s)"
-  (wp: dmo_wp modify_wp crunch_wps
-    simp: crunch_simps ignore: freeMemory
-    simp: freeMemory_def storeWord_def clearMemory_def machine_op_lift_def machine_rest_lift_def mapM_x_defsym)
-
-crunch irq_state_of_state[wp]: invoke_irq_control "\<lambda>s. P (irq_state_of_state s)"
-  (wp: dmo_wp crunch_wps
-   simp: crunch_simps setIRQTrigger_def machine_op_lift_def machine_rest_lift_def)
-
-crunch irq_state_of_state[wp]: invoke_irq_handler "\<lambda>s. P (irq_state_of_state s)"
-  (wp: dmo_wp simp: maskInterrupt_def)
-
-crunch irq_state_of_state[wp]: arch_perform_invocation "\<lambda>(s::det_state). P (irq_state_of_state s)"
-  (wp: dmo_wp modify_wp simp: set_current_pd_def invalidateLocalTLB_ASID_def invalidateLocalTLB_VAASID_def cleanByVA_PoU_def do_flush_def cache_machine_op_defs do_flush_defs wp: crunch_wps simp: crunch_simps ignore: ignore_failure)
-
-crunch irq_state_of_state[wp]: finalise_cap "\<lambda>(s::det_state). P (irq_state_of_state s)"
-  (wp: select_wp modify_wp crunch_wps dmo_wp simp: crunch_simps invalidateLocalTLB_ASID_def cleanCaches_PoU_def dsb_def invalidate_I_PoU_def clean_D_PoU_def)
-
-crunch irq_state_of_state[wp]: send_signal "\<lambda>s. P (irq_state_of_state s)"
-
-crunch irq_state_of_state[wp]: cap_swap_for_delete "\<lambda>(s::det_state). P (irq_state_of_state s)"
-
-crunch irq_state_of_state[wp]: cancel_badged_sends "\<lambda>(s::det_state). P (irq_state_of_state s)"
-  (wp: crunch_wps dmo_wp hoare_unless_wp modify_wp simp: filterM_mapM crunch_simps no_irq_clearMemory simp: clearMemory_def storeWord_def invalidateLocalTLB_ASID_def
-   ignore: filterM)
-
-crunch irq_state_of_state[wp]: restart,invoke_domain "\<lambda>(s::det_state). P (irq_state_of_state s)"
-
-subsection "reads_equiv"
-
-(* this to go in InfloFlowBase? *)
-lemma get_object_revrv:
-  "reads_equiv_valid_rv_inv (affects_equiv aag l) aag \<top>\<top> \<top> (get_object ptr)"
-  unfolding get_object_def
-  apply(rule equiv_valid_rv_bind)
-    apply(rule equiv_valid_rv_guard_imp)
-     apply(rule gets_kheap_revrv')
-    apply(simp, simp)
-   apply(rule equiv_valid_2_bind)
-      apply(rule return_ev2)
-      apply(simp)
-     apply(rule assert_ev2)
-     apply(simp)
-    apply(wpsimp)+
-  done
-
-lemma get_object_revrv':
-  "reads_equiv_valid_rv_inv (affects_equiv aag l) aag
-   (\<lambda>rv rv'. aag_can_read aag ptr \<longrightarrow> rv = rv')
-   \<top> (get_object ptr)"
-  unfolding get_object_def
-  apply(rule equiv_valid_rv_bind)
-    apply(rule equiv_valid_rv_guard_imp)
-     apply(rule gets_kheap_revrv)
-    apply(simp, simp)
-   apply(rule equiv_valid_2_bind)
-      apply(rule return_ev2)
-      apply(simp)
-     apply(rule assert_ev2)
-     apply(simp add: equiv_for_def)
-    apply(wpsimp)+
-  done
-
-lemma get_asid_pool_revrv':
-  "reads_equiv_valid_rv_inv (affects_equiv aag l) aag
-   (\<lambda>rv rv'. aag_can_read aag ptr \<longrightarrow> rv = rv')
-   \<top> (get_asid_pool ptr)"
-  unfolding get_asid_pool_def
-  apply(rule_tac W="\<lambda>rv rv'. aag_can_read aag ptr \<longrightarrow>rv = rv'" in equiv_valid_rv_bind)
-    apply(rule get_object_revrv')
-   apply(case_tac "aag_can_read aag ptr")
-    apply(simp split: kernel_object.splits)
-    apply(rule conjI | clarsimp | rule fail_ev2_l)+
-    apply(simp split: arch_kernel_obj.splits)
-    apply(rule conjI | clarsimp | rule return_ev2 | rule fail_ev2_l)+
-   apply(clarsimp simp: equiv_valid_2_def)
-   apply(case_tac rv)
-       apply(clarsimp simp: fail_def)+
-   apply(case_tac rv')
-       apply(clarsimp simp: fail_def)+
-   apply(rename_tac arch_kernel_obj arch_kernel_obj')
-   apply(case_tac arch_kernel_obj)
-      apply(case_tac arch_kernel_obj')
-         apply(clarsimp simp: fail_def return_def)+
-  apply(rule get_object_inv)
-  done
-
-lemma get_pt_revrv:
-  "reads_equiv_valid_rv_inv (affects_equiv aag l) aag \<top>\<top> \<top> (get_pt ptr)"
-  unfolding get_pt_def
-  apply(rule equiv_valid_rv_bind)
-    apply(rule get_object_revrv)
-   apply(simp)
-   apply(case_tac rv)
-       apply(simp | rule fail_ev2_l)+
-   apply(case_tac rv')
-       apply(simp | rule fail_ev2_r)+
-   apply(rename_tac arch_kernel_obj arch_kernel_obj')
-   apply(case_tac arch_kernel_obj)
-      apply(simp | rule fail_ev2_l)+
-     apply(case_tac arch_kernel_obj')
-        apply(simp | rule fail_ev2_r | rule return_ev2)+
-    apply(case_tac arch_kernel_obj')
-       apply(simp | rule fail_ev2_l)+
-  apply(rule get_object_inv)
-  done
-
-lemma set_pt_reads_respects:
-  "reads_respects aag l \<top> (set_pt ptr pt)"
-  unfolding set_pt_def
-  by (rule set_object_reads_respects)
-
-lemma get_pt_reads_respects:
-  "reads_respects aag l (K (is_subject aag ptr)) (get_pt ptr)"
-  unfolding get_pt_def
-  apply(wp get_object_rev hoare_vcg_all_lift
-       | wp (once) hoare_drop_imps | simp | wpc)+
-  done
-
-lemma store_pte_reads_respects:
-  "reads_respects aag l (K (is_subject aag (p && ~~ mask pt_bits)))
-    (store_pte p pte)"
-  unfolding store_pte_def fun_app_def
-  apply(wp set_pt_reads_respects get_pt_reads_respects)
-  apply(simp)
-  done
-
-lemma get_asid_pool_rev:
-  "reads_equiv_valid_inv A aag (K (is_subject aag ptr)) (get_asid_pool ptr)"
-  unfolding get_asid_pool_def
-  apply(wp get_object_rev | wpc | simp)+
-  done
-
-
-lemma assertE_reads_respects:
-  "reads_respects aag l \<top> (assertE P)"
-  by (rule assertE_ev)
+  by (simp add: detype_def)
 
 lemma gets_applyE:
-  "liftE (gets f) >>=E (\<lambda> f. g (f x)) = liftE (gets_apply f x) >>=E g"
-  apply(simp add: liftE_bindE)
-  apply(rule gets_apply)
+  "liftE (gets f) >>=E (\<lambda>f. g (f x)) = liftE (gets_apply f x) >>=E g"
+  apply (simp add: liftE_bindE)
+  apply (rule gets_apply)
   done
 
 lemma aag_can_read_own_asids:
   "is_subject_asid aag asid \<Longrightarrow> aag_can_read_asid aag asid"
   by simp
 
-lemma get_asid_pool_revrv:
-  "reads_equiv_valid_rv_inv (affects_equiv aag l) aag
-         (\<lambda>rv rv'. rv (ucast asid) = rv' (ucast asid))
-         (\<lambda>s. Some a = arm_asid_table (arch_state s) (asid_high_bits_of asid) \<and>
-          is_subject_asid aag asid \<and> asid \<noteq> 0)
-         (get_asid_pool a)"
-  unfolding get_asid_pool_def
-  apply(rule equiv_valid_rv_guard_imp)
-   apply(rule_tac R'="\<lambda> rv rv'.
-                         \<forall> asid_pool asid_pool'.
-                            rv = ArchObj (ASIDPool asid_pool) \<and> rv' = ArchObj (ASIDPool asid_pool')
-                            \<longrightarrow> asid_pool (ucast asid) = asid_pool' (ucast asid)"
-              and P="\<lambda>s. Some a = arm_asid_table (arch_state s) (asid_high_bits_of asid) \<and>
-                         is_subject_asid aag asid \<and> asid \<noteq> 0"
-              and P'="\<lambda>s. Some a = arm_asid_table (arch_state s) (asid_high_bits_of asid) \<and>
-                          is_subject_asid aag asid \<and> asid \<noteq> 0"
-               in equiv_valid_2_bind)
-      apply(clarsimp split: kernel_object.splits arch_kernel_obj.splits
-                      simp: fail_ev2_l fail_ev2_r return_ev2)
-     apply(clarsimp simp: get_object_def gets_def assert_def bind_def put_def get_def
-                          equiv_valid_2_def return_def fail_def
-                   split: if_split)
-     apply(erule reads_equivE)
-     apply(clarsimp simp: equiv_asids_def equiv_asid_def asid_pool_at_kheap)
-     apply(drule aag_can_read_own_asids)
-     apply(drule_tac s="Some a" in sym)
-     apply force
-    apply (wp wp_post_taut | simp)+
-  done
-
-lemma asid_high_bits_0_eq_1:
-  "asid_high_bits_of 0 = asid_high_bits_of 1"
-  by (auto simp: asid_high_bits_of_def asid_low_bits_def)
-
-
-
-lemma requiv_arm_asid_table_asid_high_bits_of_asid_eq:
-  "\<lbrakk>is_subject_asid aag asid; reads_equiv aag s t; asid \<noteq> 0\<rbrakk> \<Longrightarrow>
-               arm_asid_table (arch_state s) (asid_high_bits_of asid) =
-               arm_asid_table (arch_state t) (asid_high_bits_of asid)"
-  apply(erule reads_equivE)
-  apply(fastforce simp: equiv_asids_def equiv_asid_def intro: aag_can_read_own_asids)
-  done
-
-lemma find_pd_for_asid_reads_respects:
-  "reads_respects aag l (K (is_subject_asid aag asid)) (find_pd_for_asid asid)"
-  apply(simp add: find_pd_for_asid_def)
-  apply(subst gets_applyE)
-  (* everything up to and including get_asid_pool, both executions are the same.
-     it is only get_asid_pool that can return different values and for which we need
-     to go equiv_valid_2. We rewrite using associativity to make the decomposition
-     easier *)
-  apply(subst bindE_assoc[symmetric])+
-  apply(simp add: equiv_valid_def2)
-  apply(subst rel_sum_comb_equals[symmetric])
-  apply(rule equiv_valid_rv_guard_imp)
-   apply(rule_tac R'="\<lambda> rv rv'. rv (ucast asid) = rv' (ucast asid)" and Q="\<top>\<top>" and Q'="\<top>\<top>"
-               in equiv_valid_2_bindE)
-      apply(clarsimp split: option.splits simp: throwError_def returnOk_def)
-      apply(intro conjI impI allI)
-       apply(rule return_ev2, simp)
-      apply(rule return_ev2, simp)
-     apply wp+
-   apply(rule_tac R'="(=)"
-              and Q="\<lambda> rv s. rv = (arm_asid_table (arch_state s)) (asid_high_bits_of asid)
-                           \<and> is_subject_asid aag asid \<and> asid \<noteq> 0"
-              and Q'="\<lambda> rv s. rv = (arm_asid_table (arch_state s)) (asid_high_bits_of asid)
-                            \<and> is_subject_asid aag asid \<and> asid \<noteq> 0"
-               in equiv_valid_2_bindE)
-      apply (simp add: equiv_valid_def2[symmetric])
-      apply (split option.splits)
-      apply (intro conjI impI allI)
-       apply (simp add: throwError_def)
-       apply (rule return_ev2, simp)
-      apply(rule equiv_valid_2_liftE)
-      apply(clarsimp)
-      apply(rule get_asid_pool_revrv)
-     apply(wp gets_apply_wp)+
-   apply(subst rel_sum_comb_equals)
-   apply(subst equiv_valid_def2[symmetric])
-   apply(wp gets_apply_ev | simp)+
-  apply(fastforce intro: requiv_arm_asid_table_asid_high_bits_of_asid_eq)
-  done
-
-lemma find_pd_for_asid_assert_reads_respects:
-  "reads_respects aag l (pas_refined aag and pspace_aligned and valid_vspace_objs and
-    K (is_subject_asid aag asid))
-  (find_pd_for_asid_assert asid)"
-  unfolding find_pd_for_asid_assert_def
-  apply(wp get_pde_rev find_pd_for_asid_reads_respects hoare_vcg_all_lift
-       | wpc | simp)+
-   apply(rule_tac Q'="\<lambda>rv s. is_subject aag (lookup_pd_slot rv 0 && ~~ mask pd_bits)"
-               in hoare_post_imp_R)
-   apply(rule find_pd_for_asid_pd_slot_authorised)
-   apply(subgoal_tac "lookup_pd_slot r 0 = r")
-    apply(fastforce)
-   apply(simp add: lookup_pd_slot_def)
-  apply(fastforce)
-  done
-
-lemma modify_arm_hwasid_table_reads_respects:
-  "reads_respects aag l \<top> (modify
-          (\<lambda>s. s\<lparr>arch_state := arch_state s\<lparr>arm_hwasid_table := param\<rparr>\<rparr>))"
-  apply(simp add: equiv_valid_def2)
-  apply(rule modify_ev2)
-  (* FIXME: slow 5s *)
-  by(auto simp: reads_equiv_def affects_equiv_def states_equiv_for_def equiv_for_def
-          intro: equiv_asids_triv split: if_splits)
-
-
-lemma modify_arm_asid_map_reads_respects:
-  "reads_respects aag l \<top> (modify
-          (\<lambda>s. s\<lparr>arch_state := arch_state s\<lparr>arm_asid_map := param\<rparr>\<rparr>))"
-  apply(simp add: equiv_valid_def2)
-  apply(rule modify_ev2)
-  (* FIXME: slow 5s *)
-  by(auto simp: reads_equiv_def affects_equiv_def states_equiv_for_def equiv_for_def
-          intro: equiv_asids_triv split: if_splits)
-
-lemma modify_arm_next_asid_reads_respects:
-  "reads_respects aag l \<top> (modify
-          (\<lambda>s. s\<lparr>arch_state := arch_state s\<lparr>arm_next_asid := param\<rparr>\<rparr>))"
-  apply(simp add: equiv_valid_def2)
-  apply(rule modify_ev2)
-  (* FIXME: slow 5s *)
-  by(auto simp: reads_equiv_def affects_equiv_def states_equiv_for_def equiv_for_def
-          intro: equiv_asids_triv split: if_splits)
-
-
-lemmas modify_arch_state_reads_respects =
-  modify_arm_asid_map_reads_respects
-  modify_arm_hwasid_table_reads_respects
-  modify_arm_next_asid_reads_respects
-
-lemma states_equiv_for_arm_hwasid_table_update1:
-  "states_equiv_for P Q R S (s\<lparr> arch_state := (arch_state s)\<lparr> arm_hwasid_table := Y \<rparr>\<rparr>) t
-     = states_equiv_for P Q R S s t"
-  by (clarsimp simp: states_equiv_for_def equiv_for_def equiv_asids_def equiv_asid_def
-                     asid_pool_at_kheap)
-
-lemma states_equiv_for_arm_hwasid_table_update2:
-  "states_equiv_for P Q R S t (s\<lparr> arch_state := (arch_state s)\<lparr> arm_hwasid_table := Y \<rparr>\<rparr>)
-     = states_equiv_for P Q R S t s"
-  apply(rule iffI)
-   apply(drule states_equiv_for_sym)
-   apply(rule states_equiv_for_sym)
-   apply(simp add: states_equiv_for_arm_hwasid_table_update1)
-  apply(drule states_equiv_for_sym)
-  apply(rule states_equiv_for_sym)
-  apply(simp add: states_equiv_for_arm_hwasid_table_update1)
-  done
-
-lemma states_equiv_for_arm_hwasid_table_update':
-  "states_equiv_for P Q R S t (s\<lparr> arch_state := (arch_state s)\<lparr> arm_hwasid_table := Y \<rparr>\<rparr>)
-     = states_equiv_for P Q R S t s"
-  by (rule states_equiv_for_arm_hwasid_table_update2)
-
-lemmas states_equiv_for_arm_hwasid_table_update =
-  states_equiv_for_arm_hwasid_table_update1
-  states_equiv_for_arm_hwasid_table_update2
-
-
-lemma states_equiv_for_arm_next_asid_update1:
-  "states_equiv_for P Q R S (s\<lparr> arch_state := (arch_state s)\<lparr> arm_next_asid := Y \<rparr>\<rparr>) t
-     = states_equiv_for P Q R S s t"
-  by (clarsimp simp: states_equiv_for_def equiv_for_def equiv_asids_def equiv_asid_def
-                       asid_pool_at_kheap)
-
-lemma states_equiv_for_arm_next_asid_update2:
-  "states_equiv_for P Q R S t (s\<lparr> arch_state := (arch_state s)\<lparr> arm_next_asid := X \<rparr>\<rparr>)
-     = states_equiv_for P Q R S t s"
-  by (clarsimp simp: states_equiv_for_def equiv_for_def equiv_asids_def equiv_asid_def
-                     asid_pool_at_kheap)
-
-lemmas states_equiv_for_arm_next_asid_update =
-  states_equiv_for_arm_next_asid_update1
-  states_equiv_for_arm_next_asid_update2
-
-lemma states_equiv_for_arm_asid_map_update1:
-  "states_equiv_for P Q R S (s\<lparr> arch_state := (arch_state s)\<lparr> arm_asid_map := X \<rparr>\<rparr>) t
-     = states_equiv_for P Q R S s t"
-  by (clarsimp simp: states_equiv_for_def equiv_for_def equiv_asids_def equiv_asid_def
-                     asid_pool_at_kheap)
-
-lemma states_equiv_for_arm_asid_map_update2:
-  "states_equiv_for P Q R S t (s\<lparr> arch_state := (arch_state s)\<lparr> arm_asid_map := X \<rparr>\<rparr>)
-     = states_equiv_for P Q R S t s"
-  by (clarsimp simp: states_equiv_for_def equiv_for_def equiv_asids_def equiv_asid_def
-                     asid_pool_at_kheap)
-
-lemmas states_equiv_for_arm_asid_map_update =
-  states_equiv_for_arm_asid_map_update1
-  states_equiv_for_arm_asid_map_update2
-
 (* for things that only modify parts of the state not in the state relations,
    we don't care what they read since these reads are unobservable anyway;
    however, we cannot assert anything about their return-values *)
 lemma equiv_valid_2_unobservable:
   assumes f:
-    "\<And> P Q R S X st. \<lbrace> states_equiv_for P Q R S st \<rbrace> f \<lbrace>\<lambda>_. states_equiv_for P Q R S st\<rbrace>"
+    "\<And>P Q R S st. \<lbrace>states_equiv_for P Q R S st\<rbrace> f \<lbrace>\<lambda>_. states_equiv_for P Q R S st\<rbrace>"
   assumes f':
-    "\<And> P Q R S X st. \<lbrace> states_equiv_for P Q R S st \<rbrace> f' \<lbrace>\<lambda>_. states_equiv_for P Q R S st\<rbrace>"
+    "\<And>P Q R S st. \<lbrace>states_equiv_for P Q R S st\<rbrace> f' \<lbrace>\<lambda>_. states_equiv_for P Q R S st\<rbrace>"
   assumes g:
-    "\<And> P. \<lbrace> \<lambda> s. P (cur_thread s) \<rbrace> f \<lbrace> \<lambda> rv s. P (cur_thread s) \<rbrace>"
+    "\<And>P. \<lbrace>\<lambda>s. P (cur_thread s)\<rbrace> f \<lbrace>\<lambda>rv s. P (cur_thread s)\<rbrace>"
   assumes g':
-    "\<And> P. \<lbrace> \<lambda> s. P (cur_thread s) \<rbrace> f' \<lbrace> \<lambda> rv s. P (cur_thread s) \<rbrace>"
+    "\<And>P. \<lbrace>\<lambda>s. P (cur_thread s)\<rbrace> f' \<lbrace>\<lambda>rv s. P (cur_thread s)\<rbrace>"
   assumes h:
-    "\<And> P. \<lbrace> \<lambda> s. P (cur_domain s) \<rbrace> f \<lbrace> \<lambda> rv s. P (cur_domain s) \<rbrace>"
+    "\<And>P. \<lbrace>\<lambda>s. P (cur_domain s)\<rbrace> f \<lbrace>\<lambda>rv s. P (cur_domain s)\<rbrace>"
   assumes h':
-    "\<And> P. \<lbrace> \<lambda> s. P (cur_domain s) \<rbrace> f' \<lbrace> \<lambda> rv s. P (cur_domain s) \<rbrace>"
+    "\<And>P. \<lbrace>\<lambda>s. P (cur_domain s)\<rbrace> f' \<lbrace>\<lambda>rv s. P (cur_domain s)\<rbrace>"
   assumes j:
-    "\<And> P. \<lbrace> \<lambda> s. P (scheduler_action s) \<rbrace> f \<lbrace> \<lambda> rv s. P (scheduler_action s) \<rbrace>"
+    "\<And>P. \<lbrace>\<lambda>s. P (scheduler_action s)\<rbrace> f \<lbrace>\<lambda>rv s. P (scheduler_action s)\<rbrace>"
   assumes j':
-    "\<And> P. \<lbrace> \<lambda> s. P (scheduler_action s) \<rbrace> f' \<lbrace> \<lambda> rv s. P (scheduler_action s) \<rbrace>"
+    "\<And>P. \<lbrace>\<lambda>s. P (scheduler_action s)\<rbrace> f' \<lbrace>\<lambda>rv s. P (scheduler_action s)\<rbrace>"
   assumes k:
-    "\<And> P. \<lbrace> \<lambda> s. P (work_units_completed s) \<rbrace> f \<lbrace> \<lambda> rv s. P (work_units_completed s) \<rbrace>"
+    "\<And>P. \<lbrace>\<lambda>s. P (work_units_completed s)\<rbrace> f \<lbrace>\<lambda>rv s. P (work_units_completed s)\<rbrace>"
   assumes k':
-    "\<And> P. \<lbrace> \<lambda> s. P (work_units_completed s) \<rbrace> f' \<lbrace> \<lambda> rv s. P (work_units_completed s) \<rbrace>"
+    "\<And>P. \<lbrace>\<lambda>s. P (work_units_completed s)\<rbrace> f' \<lbrace>\<lambda>rv s. P (work_units_completed s)\<rbrace>"
   assumes l:
-    "\<And> P. \<lbrace> \<lambda> s. P (irq_state (machine_state s)) \<rbrace> f \<lbrace> \<lambda> rv s. P (irq_state (machine_state s)) \<rbrace>"
+    "\<And>P. \<lbrace>\<lambda>s. P (irq_state (machine_state s))\<rbrace> f \<lbrace>\<lambda>rv s. P (irq_state (machine_state s))\<rbrace>"
   assumes l':
-    "\<And> P. \<lbrace> \<lambda> s. P (irq_state (machine_state s)) \<rbrace> f' \<lbrace> \<lambda> rv s. P (irq_state (machine_state s)) \<rbrace>"
-
+    "\<And>P. \<lbrace>\<lambda>s. P (irq_state (machine_state s))\<rbrace> f' \<lbrace>\<lambda>rv s. P (irq_state (machine_state s))\<rbrace>"
   shows
     "equiv_valid_2 (reads_equiv aag) (affects_equiv aag l) (affects_equiv aag l) \<top>\<top> \<top> \<top> f f'"
-  apply(clarsimp simp: equiv_valid_2_def)
-  apply(frule use_valid[OF _ f])
-   apply(rule states_equiv_for_refl)
-  apply(frule use_valid[OF _ f'])
-   apply(rule states_equiv_for_refl)
-  apply(frule use_valid[OF _ f])
-   apply(rule states_equiv_for_refl)
-  apply(frule use_valid[OF _ f'])
-   apply(rule states_equiv_for_refl)
-  apply(frule use_valid)
-    apply(rule_tac P="(=) (cur_thread s)" in g)
-   apply(rule refl)
-  apply(frule_tac f=f' in use_valid)
-    apply(rule_tac P="(=) (cur_thread t)" in g')
-   apply(rule refl)
-  apply(frule use_valid)
-    apply(rule_tac P="(=) (cur_domain s)" in h)
-   apply(rule refl)
-  apply(frule_tac f=f' in use_valid)
-    apply(rule_tac P="(=) (cur_domain t)" in h')
-   apply(rule refl)
-  apply(frule use_valid)
-    apply(rule_tac P="(=) (scheduler_action s)" in j)
-   apply(rule refl)
-  apply(frule_tac f=f' in use_valid)
-    apply(rule_tac P="(=) (scheduler_action t)" in j')
-   apply(rule refl)
-  apply(frule use_valid)
-    apply(rule_tac P="(=) (work_units_completed s)" in k)
-   apply(rule refl)
-  apply(frule_tac f=f' in use_valid)
-    apply(rule_tac P="(=) (work_units_completed t)" in k')
-   apply(rule refl)
-  apply(frule use_valid)
-    apply(rule_tac P="(=) (irq_state (machine_state s))" in l)
-   apply(rule refl)
-  apply(frule_tac f=f' in use_valid)
-    apply(rule_tac P="(=) (irq_state (machine_state t))" in l')
-   apply(rule refl)
-
-  apply(clarsimp simp: reads_equiv_def2 affects_equiv_def2)
-  apply(auto intro: states_equiv_for_sym states_equiv_for_trans)
+  apply (clarsimp simp: equiv_valid_2_def)
+  apply (frule use_valid[OF _ f])
+   apply (rule states_equiv_for_refl)
+  apply (frule use_valid[OF _ f'])
+   apply (rule states_equiv_for_refl)
+  apply (frule use_valid[OF _ f])
+   apply (rule states_equiv_for_refl)
+  apply (frule use_valid[OF _ f'])
+   apply (rule states_equiv_for_refl)
+  apply (frule use_valid)
+    apply (rule_tac P="(=) (cur_thread s)" in g)
+   apply (rule refl)
+  apply (frule_tac f=f' in use_valid)
+    apply (rule_tac P="(=) (cur_thread t)" in g')
+   apply (rule refl)
+  apply (frule use_valid)
+    apply (rule_tac P="(=) (cur_domain s)" in h)
+   apply (rule refl)
+  apply (frule_tac f=f' in use_valid)
+    apply (rule_tac P="(=) (cur_domain t)" in h')
+   apply (rule refl)
+  apply (frule use_valid)
+    apply (rule_tac P="(=) (scheduler_action s)" in j)
+   apply (rule refl)
+  apply (frule_tac f=f' in use_valid)
+    apply (rule_tac P="(=) (scheduler_action t)" in j')
+   apply (rule refl)
+  apply (frule use_valid)
+    apply (rule_tac P="(=) (work_units_completed s)" in k)
+   apply (rule refl)
+  apply (frule_tac f=f' in use_valid)
+    apply (rule_tac P="(=) (work_units_completed t)" in k')
+   apply (rule refl)
+  apply (frule use_valid)
+    apply (rule_tac P="(=) (irq_state (machine_state s))" in l)
+   apply (rule refl)
+  apply (frule_tac f=f' in use_valid)
+    apply (rule_tac P="(=) (irq_state (machine_state t))" in l')
+   apply (rule refl)
+  apply (clarsimp simp: reads_equiv_def2 affects_equiv_def2)
+  apply (auto intro: states_equiv_for_sym states_equiv_for_trans)
   done
-
-
-crunch states_equiv_for: invalidate_hw_asid_entry "states_equiv_for P Q R S st"
-  (simp: states_equiv_for_arm_hwasid_table_update)
-
-crunch states_equiv_for: invalidate_asid "states_equiv_for P Q R S st"
-  (simp: states_equiv_for_arm_asid_map_update)
-
-lemma mol_states_equiv_for:
-  "\<lbrace>\<lambda>ms. states_equiv_for P Q R S st (s\<lparr>machine_state := ms\<rparr>)\<rbrace> machine_op_lift mop \<lbrace>\<lambda>a b. states_equiv_for P Q R S st (s\<lparr>machine_state := b\<rparr>)\<rbrace>"
-  unfolding machine_op_lift_def
-  apply (simp add: machine_rest_lift_def split_def)
-  apply (wp modify_wp)
-  apply (clarsimp simp: states_equiv_for_def)
-  apply (clarsimp simp: equiv_asids_def equiv_asid_def)
-  apply (fastforce elim!: equiv_forE intro!: equiv_forI)
-  done
-
-lemma do_machine_op_mol_states_equiv_for:
-  "invariant (do_machine_op (machine_op_lift f)) (states_equiv_for P Q R S st)"
-  apply(simp add: do_machine_op_def)
-  apply(wp modify_wp | simp add: split_def)+
-  apply(clarify)
-  apply(erule use_valid)
-   apply simp
-   apply(rule mol_states_equiv_for)
-  by simp
-
-
-(* we don't care about the relationship between virtual and hardware asids at all --
-   these should be unobservable, so rightly we don't expect this one to satisfy
-   reads_respects but instead the weaker property where we assert no relation on
-   the return values *)
-lemma find_free_hw_asid_revrv:
-  "reads_equiv_valid_rv_inv (affects_equiv aag l) aag \<top>\<top> \<top> (find_free_hw_asid)"
-  unfolding find_free_hw_asid_def fun_app_def invalidateLocalTLB_ASID_def
-  apply(rule equiv_valid_2_unobservable)
-     apply (wp modify_wp invalidate_hw_asid_entry_states_equiv_for
-               do_machine_op_mol_states_equiv_for
-               invalidate_asid_states_equiv_for dmo_wp
-           | wpc
-           | simp add: states_equiv_for_arm_asid_map_update
-                       states_equiv_for_arm_hwasid_table_update
-                       states_equiv_for_arm_next_asid_update)+
-  done
-
-lemma load_hw_asid_revrv:
-  "reads_equiv_valid_rv_inv (affects_equiv aag l) aag \<top>\<top> \<top> (load_hw_asid asid)"
-
-  apply(rule equiv_valid_2_unobservable)
-     apply(simp add: load_hw_asid_def | wp)+
-  done
-
-lemma states_equiv_for_arch_update1:
-  "\<lbrakk>arm_globals_frame A = arm_globals_frame (arch_state s);
-    arm_asid_table A = arm_asid_table (arch_state s)\<rbrakk> \<Longrightarrow>
-    states_equiv_for P Q R S (s\<lparr> arch_state := A\<rparr>) t =
-    states_equiv_for P Q R S s t"
-  apply(clarsimp simp: states_equiv_for_def equiv_for_def equiv_asids_def equiv_asid_def asid_pool_at_kheap)
-  done
-
-lemma states_equiv_for_arch_update2:
-  "\<lbrakk>arm_globals_frame A = arm_globals_frame (arch_state s);
-    arm_asid_table A = arm_asid_table (arch_state s)\<rbrakk> \<Longrightarrow>
-    states_equiv_for P Q R S t (s\<lparr> arch_state := A\<rparr>) =
-    states_equiv_for P Q R S t s"
-  apply(rule iffI)
-   apply(drule states_equiv_for_sym)
-   apply(rule states_equiv_for_sym)
-   apply(simp add: states_equiv_for_arch_update1)
-  apply(drule states_equiv_for_sym)
-  apply(rule states_equiv_for_sym)
-  apply(simp add: states_equiv_for_arch_update1)
-  done
-
-lemmas states_equiv_for_arch_update = states_equiv_for_arch_update1 states_equiv_for_arch_update2
-
-crunch states_equiv_for: store_hw_asid "states_equiv_for P Q R S st"
-  (simp: states_equiv_for_arch_update)
-
-lemma find_free_hw_asid_states_equiv_for:
-  "invariant (find_free_hw_asid) (states_equiv_for P Q R S st)"
-  apply(simp add: find_free_hw_asid_def)
-  apply(wp modify_wp invalidate_hw_asid_entry_states_equiv_for do_machine_op_mol_states_equiv_for invalidate_asid_states_equiv_for | wpc | simp add: states_equiv_for_arm_next_asid_update invalidateLocalTLB_ASID_def)+
-  done
-
-crunch states_equiv_for: get_hw_asid "states_equiv_for P Q R S st"
 
 lemma reads_respects_unobservable_unit_return:
   assumes f:
-    "\<And> P Q R S st. \<lbrace> states_equiv_for P Q R S st \<rbrace> f \<lbrace>\<lambda>_. states_equiv_for P Q R S st\<rbrace>"
+    "\<And>P Q R S st. \<lbrace>states_equiv_for P Q R S st\<rbrace> f \<lbrace>\<lambda>_. states_equiv_for P Q R S st\<rbrace>"
   assumes g:
-    "\<And> P. \<lbrace> \<lambda> s. P (cur_thread s) \<rbrace> f \<lbrace> \<lambda> rv s. P (cur_thread s) \<rbrace>"
+    "\<And>P. \<lbrace>\<lambda>s. P (cur_thread s)\<rbrace> f \<lbrace>\<lambda>rv s. P (cur_thread s)\<rbrace>"
   assumes h:
-    "\<And> P. \<lbrace> \<lambda> s. P (cur_domain s) \<rbrace> f \<lbrace> \<lambda> rv s. P (cur_domain s) \<rbrace>"
+    "\<And>P. \<lbrace>\<lambda>s. P (cur_domain s)\<rbrace> f \<lbrace>\<lambda>rv s. P (cur_domain s)\<rbrace>"
   assumes j:
-    "\<And> P. \<lbrace> \<lambda> s. P (scheduler_action s) \<rbrace> f \<lbrace> \<lambda> rv s. P (scheduler_action s) \<rbrace>"
+    "\<And>P. \<lbrace>\<lambda>s. P (scheduler_action s)\<rbrace> f \<lbrace>\<lambda>rv s. P (scheduler_action s)\<rbrace>"
   assumes k:
-    "\<And> P. \<lbrace> \<lambda> s. P (work_units_completed s) \<rbrace> f \<lbrace> \<lambda> rv s. P (work_units_completed s) \<rbrace>"
+    "\<And>P. \<lbrace>\<lambda>s. P (work_units_completed s)\<rbrace> f \<lbrace>\<lambda>rv s. P (work_units_completed s)\<rbrace>"
   assumes l:
-    "\<And> P. \<lbrace> \<lambda> s. P (irq_state_of_state s) \<rbrace> f \<lbrace> \<lambda> rv s. P (irq_state_of_state s) \<rbrace>"
-
+    "\<And>P. \<lbrace>\<lambda>s. P (irq_state_of_state s)\<rbrace> f \<lbrace>\<lambda>rv s. P (irq_state_of_state s)\<rbrace>"
   shows
     "reads_respects aag l \<top> (f::(unit,det_ext) s_monad)"
-  apply(subgoal_tac "reads_equiv_valid_rv_inv (affects_equiv aag l) aag \<top>\<top> \<top> f")
-   apply(clarsimp simp: equiv_valid_2_def equiv_valid_def2)
-  apply(rule equiv_valid_2_unobservable[OF f f g g h h j j k k l l])
+  apply (subgoal_tac "reads_equiv_valid_rv_inv (affects_equiv aag l) aag \<top>\<top> \<top> f")
+   apply (clarsimp simp: equiv_valid_2_def equiv_valid_def2)
+  apply (rule equiv_valid_2_unobservable[OF f f g g h h j j k k l l])
   done
 
 lemma dmo_mol_irq_state_of_state[wp]:
-  "\<And>P. \<lbrace>\<lambda>s. P (irq_state_of_state s) \<rbrace> do_machine_op (machine_op_lift m)
-       \<lbrace>\<lambda>_ s. P (irq_state_of_state s) \<rbrace>"
-  apply(wp dmo_wp | simp)+
-  done
-
-lemma arm_context_switch_reads_respects:
-  "reads_respects aag l \<top> (arm_context_switch pd asid)"
-  unfolding arm_context_switch_def
-  apply(rule equiv_valid_guard_imp)
-  apply(rule reads_respects_unobservable_unit_return)
-    apply (wp do_machine_op_mol_states_equiv_for get_hw_asid_states_equiv_for
-     | simp add: set_current_pd_def dsb_def isb_def writeTTBR0_def dmo_bind_valid setHardwareASID_def)+
-  done
-
-lemma arm_context_switch_states_equiv_for:
-  "invariant (arm_context_switch pd asid) (states_equiv_for P Q R S st)"
-  unfolding arm_context_switch_def
-  apply (wp do_machine_op_mol_states_equiv_for get_hw_asid_states_equiv_for | simp add: setHardwareASID_def dmo_bind_valid set_current_pd_def dsb_def isb_def writeTTBR0_def)+
-  done
-
-lemma set_vm_root_states_equiv_for[wp]:
-  "invariant (set_vm_root thread) (states_equiv_for P Q R S st)"
-  unfolding set_vm_root_def catch_def fun_app_def set_current_pd_def isb_def dsb_def writeTTBR0_def
-  apply (wp (once) hoare_drop_imps
-        |wp do_machine_op_mol_states_equiv_for hoare_vcg_all_lift arm_context_switch_states_equiv_for hoare_whenE_wp
-        | wpc | simp add: dmo_bind_valid if_apply_def2)+
-  done
-
-lemma set_vm_root_reads_respects:
-  "reads_respects aag l \<top> (set_vm_root tcb)"
-  by (rule reads_respects_unobservable_unit_return) wp+
-
-lemma get_pte_reads_respects:
-  "reads_respects aag l (K (is_subject aag (ptr && ~~ mask pt_bits))) (get_pte ptr)"
-  unfolding get_pte_def fun_app_def
-  by (wpsimp wp: get_pt_reads_respects)
-
-lemma gets_cur_thread_revrv:
-  "reads_equiv_valid_rv_inv (affects_equiv aag l) aag (=) \<top> (gets cur_thread)"
-  apply(rule equiv_valid_rv_guard_imp)
-   apply(rule gets_evrv)
-  apply(fastforce simp: equiv_for_comp[symmetric] equiv_for_or or_comp_dist elim: reads_equivE affects_equivE)
-  done
-
-crunch states_equiv_for: set_vm_root_for_flush "states_equiv_for P Q R S st"
-  (wp: do_machine_op_mol_states_equiv_for ignore: do_machine_op simp: set_current_pd_def)
-
-lemma set_vm_root_for_flush_reads_respects:
-  "reads_respects aag l (is_subject aag \<circ> cur_thread)
-    (set_vm_root_for_flush pd asid)"
-  unfolding set_vm_root_for_flush_def fun_app_def set_current_pd_def
-  apply(rule equiv_valid_guard_imp)
-  apply (wp (once) hoare_drop_imps
-        |wp arm_context_switch_reads_respects dmo_mol_reads_respects
-            hoare_vcg_all_lift gets_cur_thread_ev get_cap_rev
-        |wpc)+
-  apply (clarsimp simp: reads_equiv_def)
-  done
-
-crunch states_equiv_for: flush_table "states_equiv_for P Q R S st"
-  (wp: crunch_wps do_machine_op_mol_states_equiv_for ignore: do_machine_op simp: invalidateLocalTLB_ASID_def crunch_simps)
-
-crunch sched_act: flush_table "\<lambda> s. P (scheduler_action s)"
-  (wp: crunch_wps simp: crunch_simps)
-
-crunch wuc: flush_table "\<lambda> s. P (work_units_completed s)"
-  (wp: crunch_wps simp: crunch_simps)
-
-lemma flush_table_reads_respects:
-  "reads_respects aag l \<top> (flush_table pd asid vptr pt)"
-  apply(rule reads_respects_unobservable_unit_return)
-       apply(rule flush_table_states_equiv_for)
-      apply(rule flush_table_cur_thread)
-     apply(rule flush_table_cur_domain)
-    apply(rule flush_table_sched_act)
-   apply(rule flush_table_wuc)
-  apply wp
-  done
-
-lemma page_table_mapped_reads_respects:
-  "reads_respects aag l
-    (pas_refined aag and pspace_aligned
-     and valid_vspace_objs and K (is_subject_asid aag asid))
-  (page_table_mapped asid vaddr pt)"
-  unfolding page_table_mapped_def catch_def fun_app_def
-  apply(wp get_pde_rev | wpc | simp)+
-     apply(wp find_pd_for_asid_reads_respects | simp)+
-  done
-
-
-lemma unmap_page_table_reads_respects:
-  "reads_respects aag l (pas_refined aag and pspace_aligned and valid_vspace_objs and K (is_subject_asid aag asid))
-   (unmap_page_table asid vaddr pt)"
-  unfolding unmap_page_table_def fun_app_def page_table_mapped_def
-  apply(wp find_pd_for_asid_pd_slot_authorised
-           dmo_mol_reads_respects store_pde_reads_respects get_pde_rev get_pde_wp
-           flush_table_reads_respects find_pd_for_asid_reads_respects hoare_vcg_all_lift_R catch_ev
-       | wpc | simp add: cleanByVA_PoU_def | wp (once) hoare_drop_imps)+
-  done
-
-
-lemma perform_page_table_invocation_reads_respects:
-  "reads_respects aag l (pas_refined aag and pspace_aligned and valid_vspace_objs and K (authorised_page_table_inv aag pti))
-    (perform_page_table_invocation pti)"
-  unfolding perform_page_table_invocation_def fun_app_def cleanCacheRange_PoU_def
-  apply(rule equiv_valid_guard_imp)
-  apply(wp dmo_cacheRangeOp_reads_respects dmo_mol_reads_respects store_pde_reads_respects
-           set_cap_reads_respects
-           mapM_x_ev'' store_pte_reads_respects unmap_page_table_reads_respects get_cap_rev
-       | wpc | simp add: cleanByVA_PoU_def)+
-  apply(clarsimp simp: authorised_page_table_inv_def)
-  apply(case_tac pti)
-  apply auto
-  done
-
-lemma do_flush_reads_respects:
-  "reads_respects aag l \<top> (do_machine_op (do_flush typ start end pstart))"
-  apply (rule equiv_valid_guard_imp)
-   apply (cases "typ")
-      apply (wp dmo_mol_reads_respects dmo_cacheRangeOp_reads_respects | simp add: do_flush_def cache_machine_op_defs do_flush_defs dmo_bind_ev when_def | rule conjI | clarsimp)+
-      done
-
-lemma perform_page_directory_invocation_reads_respects:
-  "reads_respects aag l (is_subject aag \<circ> cur_thread) (perform_page_directory_invocation pdi)"
-  unfolding perform_page_directory_invocation_def
-  apply (cases pdi)
-  apply (wp do_flush_reads_respects set_vm_root_reads_respects set_vm_root_for_flush_reads_respects | simp add: when_def requiv_cur_thread_eq split del: if_split | wp (once) hoare_drop_imps | clarsimp)+
-  done
+  "do_machine_op (machine_op_lift m) \<lbrace>\<lambda>s. P (irq_state_of_state s)\<rbrace>"
+  by (wpsimp wp: dmo_wp)
 
 lemma throw_on_false_reads_respects:
-  "reads_respects aag l P f \<Longrightarrow>
-  reads_respects aag l P (throw_on_false ex f)"
-  unfolding throw_on_false_def fun_app_def unlessE_def
-  apply(wp | simp)+
-  done
-
-lemma check_mapping_pptr_reads_respects:
-  "reads_respects aag l
-    (K (\<forall>x.   (tablePtr = Inl x \<longrightarrow> is_subject aag (x && ~~ mask pt_bits))
-            \<and> (tablePtr = Inr x \<longrightarrow> is_subject aag (x && ~~ mask pd_bits))))
-  (check_mapping_pptr pptr pgsz tablePtr)"
-  unfolding check_mapping_pptr_def fun_app_def
-  apply(rule equiv_valid_guard_imp)
-   apply(wp get_pte_reads_respects get_pde_rev | wpc)+
-  apply(simp)
-  done
-
-lemma lookup_pt_slot_reads_respects:
-  "reads_respects aag l (K (is_subject aag (lookup_pd_slot pd vptr && ~~ mask pd_bits))) (lookup_pt_slot pd vptr)"
-  unfolding lookup_pt_slot_def fun_app_def
-  apply(wp get_pde_rev | wpc | simp)+
-  done
-
-crunch sched_act: flush_page "\<lambda>s. P (scheduler_action s)"
-  (wp: crunch_wps simp: if_apply_def2)
-
-crunch wuc: flush_page "\<lambda>s. P (work_units_completed s)"
-  (wp: crunch_wps simp: if_apply_def2)
-
-crunch states_equiv_for: flush_page "states_equiv_for P Q R S st"
-  (wp: do_machine_op_mol_states_equiv_for crunch_wps ignore: do_machine_op simp: invalidateLocalTLB_VAASID_def if_apply_def2)
-
-lemma flush_page_reads_respects:
-  "reads_respects aag l \<top> (flush_page page_size pd asid vptr)"
-  apply (blast intro: reads_respects_unobservable_unit_return flush_page_states_equiv_for flush_page_cur_thread flush_page_cur_domain flush_page_sched_act flush_page_wuc flush_page_irq_state_of_state)
-  done
-
-(* clagged some help from unmap_page_respects in Arch_AC *)
-lemma unmap_page_reads_respects:
-  "reads_respects aag l (pas_refined aag and pspace_aligned and valid_vspace_objs and K (is_subject_asid aag asid \<and> vptr < kernel_base)) (unmap_page pgsz asid vptr pptr)"
-  unfolding unmap_page_def catch_def fun_app_def cleanCacheRange_PoU_def
-  apply (simp add: unmap_page_def swp_def cong: vmpage_size.case_cong)
-  apply(wp dmo_mol_reads_respects dmo_cacheRangeOp_reads_respects
-           store_pte_reads_respects[simplified]
-           check_mapping_pptr_reads_respects
-           throw_on_false_reads_respects  lookup_pt_slot_reads_respects
-           lookup_pt_slot_authorised lookup_pt_slot_authorised2
-           store_pde_reads_respects[simplified] flush_page_reads_respects
-           find_pd_for_asid_reads_respects find_pd_for_asid_pd_slot_authorised
-           mapM_ev''[
-                     where m = "(\<lambda>a. store_pte a InvalidPTE)"
-                       and P = "\<lambda>x s. is_subject aag (x && ~~ mask pt_bits)"]
-           mapM_ev''[where m = "(\<lambda>a. store_pde a InvalidPDE)"
-                       and P = "\<lambda>x s. is_subject aag (x && ~~ mask pd_bits)"]
-
-       | wpc
-       | simp add: is_aligned_6_masks is_aligned_mask[symmetric] cleanByVA_PoU_def
-       | wp (once) hoare_drop_imps)+
-  done
+  "reads_respects aag l P f
+   \<Longrightarrow> reads_respects aag l P (throw_on_false ex f)"
+  unfolding throw_on_false_def fun_app_def unlessE_def by wpsimp
 
 lemma dmo_mol_2_reads_respects:
   "reads_respects aag l \<top> (do_machine_op (machine_op_lift mop >>= (\<lambda> y. machine_op_lift mop')))"
-  apply(rule use_spec_ev)
-  apply(rule do_machine_op_spec_reads_respects)
-  apply wp
-     apply(rule machine_op_lift_ev)
-    apply(rule machine_op_lift_ev)
-   apply(rule wp_post_taut)
-  by (wp | simp)+
+  apply (rule use_spec_ev)
+  apply (rule do_machine_op_spec_reads_respects)
+  by (wpsimp wp: machine_op_lift_ev)+
 
 lemma tl_subseteq:
   "set (tl xs) \<subseteq> set xs"
   by (induct xs, auto)
-
-
-crunch states_equiv_for: invalidate_tlb_by_asid "states_equiv_for P Q R S st"
-  (wp: do_machine_op_mol_states_equiv_for ignore: do_machine_op simp: invalidateLocalTLB_ASID_def)
-
-
-crunch sched_act[wp]: invalidate_tlb_by_asid "\<lambda>s. P (scheduler_action s)"
-crunch wuc[wp]: invalidate_tlb_by_asid "\<lambda>s. P (work_units_completed s)"
-
-lemma invalidate_tlb_by_asid_reads_respects:
-  "reads_respects aag l (\<lambda>_. True) (invalidate_tlb_by_asid asid)"
-  apply(rule reads_respects_unobservable_unit_return)
-      apply (rule invalidate_tlb_by_asid_states_equiv_for)
-     apply wp+
-  done
-
-
-lemma get_master_pte_reads_respects:
-  "reads_respects aag l (K (is_subject aag (p && ~~ mask pt_bits))) (get_master_pte p)"
-  unfolding get_master_pte_def
-  apply(wp get_pte_reads_respects | wpc | simp
-       | wp (once) hoare_drop_imps)+
-  apply(fastforce simp: pt_bits_def pageBits_def mask_lower_twice)
-  done
-
-
-lemma get_master_pde_reads_respects:
-  "reads_respects aag l (K (is_subject aag (x && ~~ mask pd_bits))) (get_master_pde x)"
-  unfolding get_master_pde_def
-  apply(wp get_pde_rev | wpc | simp
-       | wp (once) hoare_drop_imps)+
-  apply(fastforce simp: pd_bits_def pageBits_def mask_lower_twice)
-  done
 
 
 abbreviation(input) aag_can_read_label where
@@ -834,259 +156,103 @@ abbreviation(input) aag_can_read_label where
 
 definition labels_are_invisible where
   "labels_are_invisible aag l L \<equiv>
-         (\<forall> d \<in> L. \<not> aag_can_read_label aag d) \<and>
-         (aag_can_affect_label aag l \<longrightarrow>
-              (\<forall> d \<in> L. d \<notin> subjectReads (pasPolicy aag) l))"
+     (\<forall>d \<in> L. \<not> aag_can_read_label aag d) \<and>
+     (aag_can_affect_label aag l \<longrightarrow> (\<forall>d \<in> L. d \<notin> subjectReads (pasPolicy aag) l))"
 
 
 lemma equiv_but_for_reads_equiv:
-  assumes domains_distinct: "pas_domains_distinct aag"
-  shows
-  "\<lbrakk>labels_are_invisible aag l L; equiv_but_for_labels aag L s s'\<rbrakk> \<Longrightarrow>
-   reads_equiv aag s s'"
-  apply(simp add: reads_equiv_def2)
-  apply(rule conjI)
-   apply(clarsimp simp: labels_are_invisible_def equiv_but_for_labels_def)
-   apply(rule states_equiv_forI)
-             apply(fastforce intro: equiv_forI elim: states_equiv_forE equiv_forD)+
-       apply((auto intro!: equiv_forI elim!: states_equiv_forE elim!: equiv_forD
-             |clarsimp simp: o_def)+)[1]
-      apply(fastforce intro: equiv_forI elim: states_equiv_forE equiv_forD)+
-    apply(fastforce simp: equiv_asids_def elim: states_equiv_forE elim: equiv_forD)
+  "\<lbrakk> pas_domains_distinct aag; labels_are_invisible aag l L; equiv_but_for_labels aag L s s' \<rbrakk>
+     \<Longrightarrow> reads_equiv aag s s'"
+  apply (simp add: reads_equiv_def2)
+  apply (rule conjI)
+   apply (clarsimp simp: labels_are_invisible_def equiv_but_for_labels_def)
+   apply (rule states_equiv_forI)
+            apply (fastforce intro: equiv_forI elim: states_equiv_forE equiv_forD)+
+       apply (auto intro!: equiv_forI elim!: states_equiv_forE elim!: equiv_forD simp: o_def)[1]
+      apply (fastforce intro: equiv_forI elim: states_equiv_forE equiv_forD)+
+    apply (fastforce simp: equiv_asids_def elim: states_equiv_forE elim: equiv_forD)
    apply (clarsimp simp: equiv_for_def states_equiv_for_def disjoint_iff_not_equal)
-   apply (metis domains_distinct[THEN pas_domains_distinct_inj])
-  apply(fastforce simp: equiv_but_for_labels_def)
+   apply (metis pas_domains_distinct_inj)
+  apply (fastforce simp: equiv_but_for_labels_def)
   done
 
 lemma equiv_but_for_affects_equiv:
-  assumes domains_distinct: "pas_domains_distinct aag"
-  shows
-  "\<lbrakk>labels_are_invisible aag l L; equiv_but_for_labels aag L s s'\<rbrakk> \<Longrightarrow>
-   affects_equiv aag l s s'"
-  apply(subst affects_equiv_def2)
-  apply(clarsimp simp: labels_are_invisible_def equiv_but_for_labels_def aag_can_affect_label_def)
-  apply(rule states_equiv_forI)
-         apply(fastforce intro!: equiv_forI elim!: states_equiv_forE equiv_forD)+
-   apply(fastforce simp: equiv_asids_def elim!: states_equiv_forE elim!: equiv_forD)
+  "\<lbrakk> pas_domains_distinct aag; labels_are_invisible aag l L; equiv_but_for_labels aag L s s' \<rbrakk>
+     \<Longrightarrow> affects_equiv aag l s s'"
+  apply (subst affects_equiv_def2)
+  apply (clarsimp simp: labels_are_invisible_def equiv_but_for_labels_def aag_can_affect_label_def)
+  apply (rule states_equiv_forI)
+           apply (fastforce intro!: equiv_forI elim!: states_equiv_forE equiv_forD)+
+   apply (fastforce simp: equiv_asids_def elim!: states_equiv_forE elim!: equiv_forD)
   apply (clarsimp simp: equiv_for_def states_equiv_for_def disjoint_iff_not_equal)
-  apply (metis domains_distinct[THEN pas_domains_distinct_inj])
+  apply (metis pas_domains_distinct_inj)
   done
 
 (* consider rewriting the return-value assumption using equiv_valid_rv_inv *)
 lemma ev2_invisible:
   assumes domains_distinct: "pas_domains_distinct aag"
   shows
-  "\<lbrakk>labels_are_invisible aag l L;
-    labels_are_invisible aag l L';
-    modifies_at_most aag L Q f;
-    modifies_at_most aag L' Q' g;
-    \<forall> s t. P s \<and> P' t \<longrightarrow> (\<forall>(rva,s') \<in> fst (f s). \<forall>(rvb,t') \<in> fst (g t). W rva rvb)\<rbrakk>
-  \<Longrightarrow>
-  equiv_valid_2 (reads_equiv aag) (affects_equiv aag l) (affects_equiv aag l)
-    W (P and Q) (P' and Q') f g"
-  apply(clarsimp simp: equiv_valid_2_def)
-  apply(rule conjI)
+  "\<lbrakk> labels_are_invisible aag l L; labels_are_invisible aag l L';
+     modifies_at_most aag L Q f; modifies_at_most aag L' Q' g;
+     \<forall>s t. P s \<and> P' t \<longrightarrow> (\<forall>(rva,s') \<in> fst (f s). \<forall>(rvb,t') \<in> fst (g t). W rva rvb) \<rbrakk>
+     \<Longrightarrow> equiv_valid_2 (reads_equiv aag) (affects_equiv aag l) (affects_equiv aag l)
+                        W (P and Q) (P' and Q') f g"
+  apply (clarsimp simp: equiv_valid_2_def)
+  apply (rule conjI)
    apply blast
-  apply(drule_tac s=s in modifies_at_mostD, assumption+)
-  apply(drule_tac s=t in modifies_at_mostD, assumption+)
-  apply(frule (1) equiv_but_for_reads_equiv[OF domains_distinct])
-  apply(frule_tac s=t in equiv_but_for_reads_equiv[OF domains_distinct], assumption)
-  apply(drule (1) equiv_but_for_affects_equiv[OF domains_distinct])
-  apply(drule_tac s=t in equiv_but_for_affects_equiv[OF domains_distinct], assumption)
-  apply(blast intro: reads_equiv_trans reads_equiv_sym affects_equiv_trans affects_equiv_sym)
+  apply (drule_tac s=s in modifies_at_mostD, assumption+)
+  apply (drule_tac s=t in modifies_at_mostD, assumption+)
+  apply (frule (1) equiv_but_for_reads_equiv[OF domains_distinct])
+  apply (frule_tac s=t in equiv_but_for_reads_equiv[OF domains_distinct], assumption)
+  apply (drule (1) equiv_but_for_affects_equiv[OF domains_distinct])
+  apply (drule_tac s=t in equiv_but_for_affects_equiv[OF domains_distinct], assumption)
+  apply (blast intro: reads_equiv_trans reads_equiv_sym affects_equiv_trans affects_equiv_sym)
   done
+
+lemma ev_invisible:
+  assumes domains_distinct: "pas_domains_distinct aag"
+  shows
+    "\<lbrakk> labels_are_invisible aag l L; modifies_at_most aag L Q f;
+       \<forall>s t. P s \<and> P t \<longrightarrow> (\<forall>(rva, s') \<in> fst (f s). \<forall>(rvb, t') \<in> fst(f t). W rva rvb) \<rbrakk>
+       \<Longrightarrow> equiv_valid_2 (reads_equiv aag) (affects_equiv aag l) (affects_equiv aag l)
+                         W (P and Q) (P and Q) f f"
+  by (rule ev2_invisible[OF domains_distinct]; simp)
 
 lemma modify_det:
   "det (modify f)"
-  apply(clarsimp simp: det_def modify_def get_def put_def bind_def)
-  done
+  by (clarsimp simp: det_def modify_def get_def put_def bind_def)
 
 lemma dummy_kheap_update:
-  "st = st\<lparr> kheap := kheap st \<rparr>"
+  "st = st\<lparr>kheap := kheap st\<rparr>"
   by simp
 
-(* we need to know we're not doing an asid pool update, or else this could affect
-   what some other domain sees *)
-lemma set_object_equiv_but_for_labels:
-  "\<lbrace>equiv_but_for_labels aag L st and (\<lambda> s. \<not> asid_pool_at ptr s) and
-    K ((\<forall> asid_pool. obj \<noteq> ArchObj (ASIDPool asid_pool)) \<and> pasObjectAbs aag ptr \<in> L)\<rbrace>
-   set_object ptr obj
-   \<lbrace>\<lambda>_. equiv_but_for_labels aag L st\<rbrace>"
-  apply (wpsimp wp: set_object_wp)
-  apply(clarsimp simp: equiv_but_for_labels_def)
-  apply(subst dummy_kheap_update[where st=st])
-  apply(rule states_equiv_for_non_asid_pool_kheap_update)
-     apply assumption
-    apply(fastforce intro: equiv_forI elim: states_equiv_forE equiv_forE)
-   apply(fastforce simp: non_asid_pool_kheap_update_def)
-  apply(clarsimp simp: non_asid_pool_kheap_update_def asid_pool_at_kheap)
-  done
-
-
-lemma get_tcb_not_asid_pool_at:
-  "get_tcb ref s = Some y \<Longrightarrow> \<not> asid_pool_at ref s"
-  by(fastforce simp: get_tcb_def asid_pool_at_kheap)
-
-lemma as_user_set_register_ev2:
-  assumes domains_distinct: "pas_domains_distinct aag"
-  shows
-  "labels_are_invisible aag l (pasObjectAbs aag ` {thread,thread'}) \<Longrightarrow>
-   equiv_valid_2 (reads_equiv aag) (affects_equiv aag l) (affects_equiv aag l) (=) \<top> \<top> (as_user thread (setRegister x y)) (as_user thread' (setRegister a b))"
-  apply(simp add: as_user_def)
-  apply(rule equiv_valid_2_guard_imp)
-   apply(rule_tac L="{pasObjectAbs aag thread}" and L'="{pasObjectAbs aag thread'}" and Q="\<top>" and Q'="\<top>" in ev2_invisible[OF domains_distinct])
-        apply(simp add: labels_are_invisible_def)+
-      apply((rule modifies_at_mostI | wp set_object_equiv_but_for_labels | simp add: split_def | fastforce dest: get_tcb_not_asid_pool_at)+)[2]
-    apply auto
-  done
-
-
 lemma reads_affects_equiv_kheap_eq:
-  "\<lbrakk>reads_equiv aag s s'; affects_equiv aag l s s';
-    aag_can_affect aag l x \<or> aag_can_read aag x\<rbrakk> \<Longrightarrow>
-   kheap s x = kheap s' x"
-  apply(erule disjE)
-   apply(fastforce elim: affects_equivE equiv_forE)
-  apply(fastforce elim: reads_equivE equiv_forE)
-  done
+  "\<lbrakk> reads_equiv aag s s'; affects_equiv aag l s s'; aag_can_affect aag l x \<or> aag_can_read aag x \<rbrakk>
+     \<Longrightarrow> kheap s x = kheap s' x"
+  by (fastforce elim: affects_equivE reads_equivE equiv_forE)
 
 lemma reads_affects_equiv_get_tcb_eq:
-  "\<lbrakk>aag_can_read aag thread \<or> aag_can_affect aag l thread;
-    reads_equiv aag s t; affects_equiv aag l s t\<rbrakk> \<Longrightarrow>
-   get_tcb thread s = get_tcb thread t"
-  apply (fastforce simp: get_tcb_def split: kernel_object.splits option.splits simp: reads_affects_equiv_kheap_eq)
-  done
-
-lemma as_user_set_register_reads_respects':
-  assumes domains_distinct: "pas_domains_distinct aag"
-  shows
-  "reads_respects aag l \<top> (as_user thread (setRegister x y))"
-  apply (case_tac "aag_can_read aag thread \<or> aag_can_affect aag l thread")
-   apply (simp add: as_user_def split_def)
-   apply (rule gen_asm_ev)
-   apply (wp set_object_reads_respects select_f_ev gets_the_ev)
-   apply (auto intro: reads_affects_equiv_get_tcb_eq det_setRegister)[1]
-  apply(simp add: equiv_valid_def2)
-  apply(rule as_user_set_register_ev2[OF domains_distinct])
-  apply(simp add: labels_are_invisible_def)
-  done
-
-lemma as_user_get_register_reads_respects:
-  "reads_respects aag l (K (is_subject aag thread)) (as_user thread (getRegister reg))"
-  apply (simp add: as_user_def split_def)
-  apply (wp set_object_reads_respects select_f_ev gets_the_ev)
-  apply (auto intro: reads_affects_equiv_get_tcb_eq det_getRegister)[1]
-  done
-
-lemma set_message_info_reads_respects:
-  assumes domains_distinct: "pas_domains_distinct aag"
-  shows
-  "reads_respects aag l \<top>
-    (set_message_info thread info)"
-  unfolding set_message_info_def fun_app_def
-  apply(rule as_user_set_register_reads_respects'[OF domains_distinct])
-  done
+  "\<lbrakk> aag_can_read aag t \<or> aag_can_affect aag l t; reads_equiv aag s s'; affects_equiv aag l s s' \<rbrakk>
+     \<Longrightarrow> get_tcb t s = get_tcb t s'"
+  by (fastforce simp: get_tcb_def reads_affects_equiv_kheap_eq)
 
 lemma equiv_valid_get_assert:
-  "equiv_valid_inv I A P f \<Longrightarrow>
-   equiv_valid_inv I A P (get >>= (\<lambda> s. assert (g s) >>= (\<lambda> y. f)))"
-  apply(subst equiv_valid_def2)
-  apply(rule_tac W="\<top>\<top>" in equiv_valid_rv_bind)
-    apply(rule equiv_valid_rv_guard_imp)
-     apply(rule equiv_valid_rv_trivial)
+  "equiv_valid_inv I A P f
+   \<Longrightarrow> equiv_valid_inv I A P (get >>= (\<lambda> s. assert (g s) >>= (\<lambda> y. f)))"
+  apply (subst equiv_valid_def2)
+  apply (rule_tac W="\<top>\<top>" in equiv_valid_rv_bind)
+    apply (rule equiv_valid_rv_guard_imp)
+     apply (rule equiv_valid_rv_trivial)
      apply wpsimp+
-   apply(rule_tac R'="\<top>\<top>" in equiv_valid_2_bind)
-      apply(simp add: equiv_valid_def2)
-     apply(rule assert_ev2)
+   apply (rule_tac R'="\<top>\<top>" in equiv_valid_2_bind)
+      apply (simp add: equiv_valid_def2)
+     apply (rule assert_ev2)
      apply (wp | simp)+
   done
 
-lemma store_word_offs_reads_respects:
-  "reads_respects aag l \<top> (store_word_offs ptr offs v)"
-  apply(simp add: store_word_offs_def)
-  apply(rule equiv_valid_get_assert)
-  apply(simp add: storeWord_def)
-  apply(simp add: do_machine_op_bind)
-  apply(wp)
-     apply(rule use_spec_ev)
-     apply(rule do_machine_op_spec_reads_respects)
-     apply(clarsimp simp: equiv_valid_def2 equiv_valid_2_def in_monad)
-     apply(fastforce intro: equiv_forI elim: equiv_forE)
-    apply(rule use_spec_ev | rule do_machine_op_spec_reads_respects
-         | simp add: spec_equiv_valid_def | rule assert_ev2 | wp modify_wp)+
-  done
-
-
-lemma set_mrs_reads_respects:
-  "reads_respects aag l (K (aag_can_read aag thread \<or> aag_can_affect aag l thread)) (set_mrs thread buf msgs)"
-  apply(simp add: set_mrs_def cong: option.case_cong_weak)
-  apply(wp mapM_x_ev' store_word_offs_reads_respects set_object_reads_respects
-       | wpc | simp add: split_def split del: if_split add: zipWithM_x_mapM_x)+
-  apply(auto intro: reads_affects_equiv_get_tcb_eq)
-  done
-
-lemma perform_page_invocation_reads_respects:
-  assumes domains_distinct[wp]: "pas_domains_distinct aag"
-  shows
-  "reads_respects aag l (pas_refined aag and K (authorised_page_inv aag pgi) and valid_page_inv pgi and valid_vspace_objs and pspace_aligned and is_subject aag \<circ> cur_thread) (perform_page_invocation pgi)"
-  unfolding perform_page_invocation_def fun_app_def when_def cleanCacheRange_PoU_def
-  apply(rule equiv_valid_guard_imp)
-  apply wpc
-      apply(simp add: mapM_discarded swp_def)
-      apply (wp dmo_mol_reads_respects dmo_cacheRangeOp_reads_respects
-                mapM_x_ev'' store_pte_reads_respects
-                set_cap_reads_respects mapM_ev'' store_pde_reads_respects
-                unmap_page_reads_respects set_vm_root_reads_respects
-                dmo_mol_2_reads_respects set_vm_root_for_flush_reads_respects get_cap_rev
-                do_flush_reads_respects invalidate_tlb_by_asid_reads_respects
-                get_master_pte_reads_respects get_master_pde_reads_respects
-                set_mrs_reads_respects set_message_info_reads_respects
-            | simp add: cleanByVA_PoU_def pte_check_if_mapped_def pde_check_if_mapped_def  | wpc | wp (once) hoare_drop_imps[where R="\<lambda> r s. r"])+
-  apply(clarsimp simp: authorised_page_inv_def valid_page_inv_def)
-  apply (auto simp: cte_wp_at_caps_of_state valid_slots_def cap_auth_conferred_def
-                    update_map_data_def is_page_cap_def authorised_slots_def
-                    valid_page_inv_def valid_cap_simps
-             dest!: bspec[OF _ rev_subsetD[OF _ tl_subseteq]]
-       | auto dest!: clas_caps_of_state
-               simp: cap_links_asid_slot_def label_owns_asid_slot_def
-              dest!: pas_refined_Control
-       | (frule aag_can_read_self, simp)+)+
-  done
-
-lemma equiv_asids_arm_asid_table_update:
-  "\<lbrakk>equiv_asids R s t; kheap s pool_ptr = kheap t pool_ptr\<rbrakk> \<Longrightarrow>
-   equiv_asids R (s\<lparr>arch_state := arch_state s
-                   \<lparr>arm_asid_table := arm_asid_table (arch_state s)
-                      (asid_high_bits_of asid \<mapsto> pool_ptr)\<rparr>\<rparr>)
-              (t\<lparr>arch_state := arch_state t
-                   \<lparr>arm_asid_table := arm_asid_table (arch_state t)
-                      (asid_high_bits_of asid \<mapsto> pool_ptr)\<rparr>\<rparr>)"
-  apply(clarsimp simp: equiv_asids_def equiv_asid_def asid_pool_at_kheap)
-  done
-
-
-lemma arm_asid_table_update_reads_respects:
-  "reads_respects aag l (K (is_subject aag pool_ptr))
-        (do r \<leftarrow> gets (arm_asid_table \<circ> arch_state);
-            modify
-             (\<lambda>s. s\<lparr>arch_state := arch_state s
-                      \<lparr>arm_asid_table := r(asid_high_bits_of asid \<mapsto> pool_ptr)\<rparr>\<rparr>)
-         od)"
-  apply(simp add: equiv_valid_def2)
-  apply(rule_tac W="\<top>\<top>" and Q="\<lambda> rv s. is_subject aag pool_ptr \<and> rv = arm_asid_table (arch_state s)" in equiv_valid_rv_bind)
-    apply(rule equiv_valid_rv_guard_imp[OF equiv_valid_rv_trivial])
-     apply wpsimp+
-   apply(rule modify_ev2)
-   apply clarsimp
-   apply (drule(1) is_subject_kheap_eq[rotated])
-   apply (auto simp add: reads_equiv_def2 affects_equiv_def2 states_equiv_for_def equiv_for_def intro!: equiv_asids_arm_asid_table_update)
-   done
-
-
 lemma my_bind_rewrite_lemma:
   "(f >>= g) =  (f >>= (\<lambda> r. (g r) >>= (\<lambda> x. return ())))"
-  apply simp
-  done
+  by simp
 
 lemma delete_objects_reads_respects:
   "reads_respects aag l (\<lambda>_. True) (delete_objects p b)"
@@ -1096,160 +262,8 @@ lemma delete_objects_reads_respects:
 
 lemma another_hacky_rewrite:
   "do a; (do x \<leftarrow> f; g x od); h; j od = do a; (f >>= g >>= (\<lambda>_. h)); j od"
-  apply(simp add: bind_assoc[symmetric])
-  done
+  by (simp add: bind_assoc[symmetric])
 
-lemma perform_asid_control_invocation_reads_respects:
-  notes K_bind_ev[wp del]
-  shows
-  "reads_respects aag l (K (authorised_asid_control_inv aag aci))
-  (perform_asid_control_invocation aci)"
-  unfolding perform_asid_control_invocation_def
-  apply(rule gen_asm_ev)
-  apply(rule equiv_valid_guard_imp)
-   (* we do some hacky rewriting here to separate out the bit that does interesting stuff from the rest *)
-   apply(subst (6) my_bind_rewrite_lemma)
-   apply(subst (1) bind_assoc[symmetric])
-   apply(subst another_hacky_rewrite)
-   apply(subst another_hacky_rewrite)
-   apply(wpc)
-   apply(rule bind_ev)
-     apply(rule K_bind_ev)
-     apply(rule_tac P'=\<top> in bind_ev)
-       apply(rule K_bind_ev)
-       apply(rule bind_ev)
-         apply(rule bind_ev)
-           apply(rule return_ev)
-          apply(rule K_bind_ev)
-          apply simp
-          apply(rule arm_asid_table_update_reads_respects)
-         apply (wp cap_insert_reads_respects retype_region_reads_respects
-                   set_cap_reads_respects delete_objects_reads_respects get_cap_rev
-               | simp add: authorised_asid_control_inv_def)+
-  apply(auto dest!: is_aligned_no_overflow)
-  done
-
-
-lemma set_asid_pool_reads_respects:
-  "reads_respects aag l \<top> (set_asid_pool ptr pool)"
-  unfolding set_asid_pool_def
-  by (rule set_object_reads_respects)
-
-lemma perform_asid_pool_invocation_reads_respects:
-  "reads_respects aag l (pas_refined aag and K (authorised_asid_pool_inv aag api))  (perform_asid_pool_invocation api)"
-  unfolding perform_asid_pool_invocation_def
-  apply(rule equiv_valid_guard_imp)
-   apply(wp set_asid_pool_reads_respects set_cap_reads_respects
-            get_asid_pool_rev get_cap_auth_wp[where aag=aag] get_cap_rev
-        | wpc | simp)+
-  apply(clarsimp simp: authorised_asid_pool_inv_def)
-  done
-
-lemma arch_perform_invocation_reads_respects:
-  assumes domains_distinct[wp]: "pas_domains_distinct aag"
-  shows
-  "reads_respects aag l (pas_refined aag and pspace_aligned and valid_vspace_objs and
-                         authorised_arch_inv aag ai and valid_arch_inv ai and is_subject aag \<circ> cur_thread)
-    (arch_perform_invocation ai)"
-  unfolding arch_perform_invocation_def fun_app_def
-  apply(wp perform_page_table_invocation_reads_respects perform_page_directory_invocation_reads_respects perform_page_invocation_reads_respects perform_asid_control_invocation_reads_respects perform_asid_pool_invocation_reads_respects | wpc)+
-  apply(case_tac ai)
-  apply(auto simp: authorised_arch_inv_def valid_arch_inv_def)
-  done
-
-lemma equiv_asids_arm_asid_table_delete:
-  "\<lbrakk>equiv_asids R s t\<rbrakk> \<Longrightarrow>
-   equiv_asids R (s\<lparr>arch_state := arch_state s
-                   \<lparr>arm_asid_table :=
-                        \<lambda>a. if a = asid_high_bits_of asid then None
-                             else arm_asid_table (arch_state s) a\<rparr>\<rparr>)
-              (t\<lparr>arch_state := arch_state t
-                   \<lparr>arm_asid_table :=
-                        \<lambda>a. if a = asid_high_bits_of asid then None
-                             else arm_asid_table (arch_state t) a\<rparr>\<rparr>)"
-  apply(clarsimp simp: equiv_asids_def equiv_asid_def asid_pool_at_kheap)
-  done
-
-lemma arm_asid_table_delete_ev2:
-  "equiv_valid_2 (reads_equiv aag) (affects_equiv aag l) (affects_equiv aag l)
-     \<top>\<top> (\<lambda>s. rv = arm_asid_table (arch_state s))
-        (\<lambda>s. rv' = arm_asid_table (arch_state s))
-          (modify
-             (\<lambda>s. s\<lparr>arch_state := arch_state s
-                      \<lparr>arm_asid_table :=
-                        \<lambda>a. if a = asid_high_bits_of base then None
-                             else rv a\<rparr>\<rparr>))
-          (modify
-             (\<lambda>s. s\<lparr>arch_state := arch_state s
-                      \<lparr>arm_asid_table :=
-                        \<lambda>a. if a = asid_high_bits_of base then None
-                             else rv' a\<rparr>\<rparr>))"
-  apply(rule modify_ev2)
-  (* slow 15s *)
-  by(auto simp: reads_equiv_def2 affects_equiv_def2
-          intro!: states_equiv_forI elim!: states_equiv_forE
-          intro!: equiv_forI elim!: equiv_forE
-          intro!: equiv_asids_arm_asid_table_delete
-          elim: is_subject_kheap_eq[simplified reads_equiv_def2 states_equiv_for_def, rotated])
-
-crunch states_equiv_for: invalidate_asid_entry "states_equiv_for P Q R S st"
-crunch sched_act: invalidate_asid_entry "\<lambda>s. P (scheduler_action s)"
-crunch wuc: invalidate_asid_entry "\<lambda>s. P (work_units_completed s)"
-crunch states_equiv_for: flush_space "states_equiv_for P Q R S st"
-  (wp: mol_states_equiv_for dmo_wp ignore: do_machine_op simp: invalidateLocalTLB_ASID_def cleanCaches_PoU_def dsb_def invalidate_I_PoU_def clean_D_PoU_def)
-crunch sched_act: flush_space "\<lambda>s. P (scheduler_action s)"
-crunch wuc: flush_space "\<lambda>s. P (work_units_completed s)"
-
-
-
-
-lemma requiv_arm_asid_table_asid_high_bits_of_asid_eq':
-  "\<lbrakk>(\<forall>asid'. asid' \<noteq> 0 \<and> asid_high_bits_of asid' = asid_high_bits_of base \<longrightarrow> is_subject_asid aag asid');reads_equiv aag s t\<rbrakk> \<Longrightarrow>
-    arm_asid_table (arch_state s) (asid_high_bits_of base) =
-    arm_asid_table (arch_state t) (asid_high_bits_of base)"
-  apply (insert asid_high_bits_0_eq_1)
-   apply(case_tac "base = 0")
-    apply(subgoal_tac "is_subject_asid aag 1")
-    apply simp
-    apply (rule requiv_arm_asid_table_asid_high_bits_of_asid_eq[where aag=aag])
-    apply (erule_tac x=1 in allE)
-    apply simp+
-    apply (rule requiv_arm_asid_table_asid_high_bits_of_asid_eq[where aag=aag])
-    apply (erule_tac x=base in allE)
-    apply simp+
-done
-
-
-lemma delete_asid_pool_reads_respects:
-  "reads_respects aag l (K (\<forall>asid'. asid' \<noteq> 0 \<and> asid_high_bits_of asid' = asid_high_bits_of base \<longrightarrow> is_subject_asid aag asid')) (delete_asid_pool base ptr)"
-  unfolding delete_asid_pool_def
-  apply(rule equiv_valid_guard_imp)
-   apply(rule bind_ev)
-     apply(simp)
-     apply(subst equiv_valid_def2)
-     apply(rule_tac W="\<top>\<top>" and Q="\<lambda>rv s. rv = arm_asid_table (arch_state s)
-        \<and> (\<forall>asid'. asid' \<noteq> 0 \<and> asid_high_bits_of asid' = asid_high_bits_of base \<longrightarrow> is_subject_asid aag asid')"
-                     in equiv_valid_rv_bind)
-       apply(rule equiv_valid_rv_guard_imp[OF equiv_valid_rv_trivial])
-        apply(wp, simp)
-      apply(simp add: when_def)
-      apply(clarsimp | rule conjI)+
-        apply(subst bind_assoc[symmetric])
-        apply(subst (3) bind_assoc[symmetric])
-        apply(rule equiv_valid_2_guard_imp)
-          apply(rule equiv_valid_2_bind)
-             apply(rule equiv_valid_2_bind)
-                apply(rule equiv_valid_2_unobservable)
-                           apply(wp set_vm_root_states_equiv_for)+
-               apply(rule arm_asid_table_delete_ev2)
-              apply(wp)+
-            apply(rule equiv_valid_2_unobservable)
-                       apply(wp mapM_wp' invalidate_asid_entry_states_equiv_for flush_space_states_equiv_for invalidate_asid_entry_cur_thread invalidate_asid_entry_sched_act invalidate_asid_entry_wuc flush_space_cur_thread flush_space_sched_act flush_space_wuc | clarsimp)+
-       apply( wp return_ev2 |
-              drule (1) requiv_arm_asid_table_asid_high_bits_of_asid_eq' |
-              clarsimp   | rule conjI |
-              simp add: equiv_valid_2_def )+
-done
 
 definition states_equal_except_kheap_asid :: "det_state \<Rightarrow> det_state \<Rightarrow> bool" where
   "states_equal_except_kheap_asid s s' \<equiv>
@@ -1267,1169 +281,231 @@ definition states_equal_except_kheap_asid :: "det_state \<Rightarrow> det_state 
      work_units_completed s = work_units_completed s' \<and>
      irq_state_of_state s = irq_state_of_state s'"
 
-lemma set_asid_pool_state_equal_except_kheap:
-  "((), s') \<in> fst (set_asid_pool ptr pool s) \<Longrightarrow>
-    states_equal_except_kheap_asid s s' \<and>
-    (\<forall>p. p \<noteq> ptr \<longrightarrow> kheap s p = kheap s' p) \<and>
-    kheap s' ptr = Some (ArchObj (ASIDPool pool)) \<and>
-    (\<forall>asid. asid \<noteq> 0 \<longrightarrow>
-      arm_asid_table (arch_state s) (asid_high_bits_of asid) =
-      arm_asid_table (arch_state s') (asid_high_bits_of asid) \<and>
-      (\<forall>pool_ptr. arm_asid_table (arch_state s) (asid_high_bits_of asid) =
-        Some pool_ptr \<longrightarrow>
-          asid_pool_at pool_ptr s = asid_pool_at pool_ptr s' \<and>
-          (\<forall>asid_pool asid_pool'. pool_ptr \<noteq> ptr \<longrightarrow>
-            kheap s pool_ptr = Some (ArchObj (ASIDPool asid_pool)) \<and>
-            kheap s' pool_ptr = Some (ArchObj (ASIDPool asid_pool')) \<longrightarrow>
-              asid_pool (ucast asid) = asid_pool' (ucast asid))))"
-  by (clarsimp simp: set_asid_pool_def put_def bind_def set_object_def get_object_def gets_def
-                     get_def return_def assert_def fail_def states_equal_except_kheap_asid_def
-                     equiv_for_def obj_at_def
-              split: if_split_asm)
-
-lemma set_asid_pool_delete_ev2:
-  "equiv_valid_2 (reads_equiv aag) (affects_equiv aag l) (affects_equiv aag l)
-     \<top>\<top> (\<lambda>s. arm_asid_table (arch_state s) (asid_high_bits_of asid) = Some a \<and>
-            kheap s a = Some (ArchObj (ASIDPool pool)) \<and>
-            asid \<noteq> 0 \<and> is_subject_asid aag asid)
-        (\<lambda>s. arm_asid_table (arch_state s) (asid_high_bits_of asid) = Some a \<and>
-            kheap s a = Some (ArchObj (ASIDPool pool')) \<and>
-            asid \<noteq> 0 \<and> is_subject_asid aag asid)
-          (set_asid_pool a (pool(ucast asid := None)))
-          (set_asid_pool a (pool'(ucast asid := None)))"
-  apply(clarsimp simp: equiv_valid_2_def)
-  apply(frule_tac s'=b in set_asid_pool_state_equal_except_kheap)
-  apply(frule_tac s'=ba in set_asid_pool_state_equal_except_kheap)
-  apply(clarsimp simp: states_equal_except_kheap_asid_def)
-  apply(rule conjI)
-   apply(clarsimp simp: states_equiv_for_def reads_equiv_def equiv_for_def | rule conjI)+
-     apply(case_tac "x=a")
-      apply(clarsimp)
-     apply(fastforce)
-    apply(clarsimp simp: equiv_asids_def equiv_asid_def | rule conjI)+
-     apply(case_tac "pool_ptr = a")
-      apply(clarsimp)
-      apply(erule_tac x="pasASIDAbs aag asid" in ballE)
-       apply(clarsimp)
-       apply(erule_tac x=asid in allE)+
-       apply(clarsimp)
-      apply(drule aag_can_read_own_asids, simp)
-     apply(erule_tac x="pasASIDAbs aag asida" in ballE)
-      apply(clarsimp)
-      apply(erule_tac x=asida in allE)+
-      apply(clarsimp)
-     apply(clarsimp)
-    apply(clarsimp)
-    apply(case_tac "pool_ptr=a")
-     apply(erule_tac x="pasASIDAbs aag asida" in ballE)
-      apply(clarsimp)+
-  apply(clarsimp simp: affects_equiv_def equiv_for_def states_equiv_for_def | rule conjI)+
-   apply(case_tac "x=a")
-    apply(clarsimp)
-   apply(fastforce)
-  apply(clarsimp simp: equiv_asids_def equiv_asid_def | rule conjI)+
-   apply(case_tac "pool_ptr=a")
-    apply(clarsimp)
-    apply(erule_tac x=asid in allE)+
-    apply(clarsimp simp: asid_pool_at_kheap)
-   apply(erule_tac x=asida in allE)+
-   apply(clarsimp)
-  apply(clarsimp)
-  apply(case_tac "pool_ptr=a")
-   apply(clarsimp)+
-  done
-
-lemma delete_asid_reads_respects:
-  "reads_respects aag l (K (asid \<noteq> 0 \<and> is_subject_asid aag asid))
-    (delete_asid asid pd)"
-  unfolding delete_asid_def
-  apply(subst equiv_valid_def2)
-  apply(rule_tac W="\<top>\<top>" and Q="\<lambda>rv s. rv = arm_asid_table (arch_state s)
-        \<and> is_subject_asid aag asid \<and> asid \<noteq> 0" in equiv_valid_rv_bind)
-    apply(rule equiv_valid_rv_guard_imp[OF equiv_valid_rv_trivial])
-     apply(wp, simp)
-   apply(case_tac "rv (asid_high_bits_of asid) =
-                   rv' (asid_high_bits_of asid)")
-    apply(simp)
-    apply(case_tac "rv' (asid_high_bits_of asid)")
-     apply(simp)
-     apply(wp return_ev2, simp)
-    apply(simp)
-    apply(rule equiv_valid_2_guard_imp)
-    apply(rule_tac R'="\<lambda>rv rv'. rv (ucast asid) = rv' (ucast asid)"
-                in equiv_valid_2_bind)
-       apply(simp add: when_def)
-       apply(clarsimp | rule conjI)+
-        apply(rule_tac R'="\<top>\<top>" in equiv_valid_2_bind)
-           apply(rule_tac R'="\<top>\<top>" in equiv_valid_2_bind)
-              apply(rule_tac R'="\<top>\<top>" in equiv_valid_2_bind)
-                 apply(subst equiv_valid_def2[symmetric])
-                 apply(rule reads_respects_unobservable_unit_return)
-                  apply(wp set_vm_root_states_equiv_for)+
-                apply(rule set_asid_pool_delete_ev2)
-               apply(wp)+
-             apply(rule equiv_valid_2_unobservable)
-                apply(wp invalidate_asid_entry_states_equiv_for
-                         invalidate_asid_entry_cur_thread)+
-            apply(simp add: invalidate_asid_entry_def
-                | wp invalidate_asid_kheap invalidate_hw_asid_entry_kheap
-                     load_hw_asid_kheap)+
-          apply(rule equiv_valid_2_unobservable)
-             apply(wp flush_space_states_equiv_for flush_space_cur_thread)+
-         apply(wp load_hw_asid_kheap | simp add: flush_space_def | wpc)+
-       apply(clarsimp | rule return_ev2)+
-      apply(rule equiv_valid_2_guard_imp)
-        apply(wp get_asid_pool_revrv)
-       apply(simp)+
-     apply(wp)+
-   apply(clarsimp simp: obj_at_def)+
-   apply(clarsimp simp: equiv_valid_2_def reads_equiv_def equiv_asids_def equiv_asid_def states_equiv_for_def)
-   apply(erule_tac x="pasASIDAbs aag asid" in ballE)
-    apply(clarsimp)
-   apply(drule aag_can_read_own_asids)
-   apply(clarsimp | wpsimp)+
-   done
-
-
-subsection "globals_equiv"
-
-
-lemma set_simple_ko_globals_equiv:
-  "\<lbrace>globals_equiv s and valid_ko_at_arm\<rbrace> set_simple_ko f ptr ep \<lbrace>\<lambda>_. globals_equiv s\<rbrace>"
-  unfolding set_simple_ko_def
-  apply(wpsimp wp: set_object_globals_equiv[THEN hoare_set_object_weaken_pre] get_object_wp
-             simp: partial_inv_def)+
-  apply(fastforce simp: obj_at_def valid_ko_at_arm_def)
-  done
-
-lemma set_endpoint_valid_ko_at_arm[wp]:
-  "\<lbrace>valid_ko_at_arm\<rbrace> set_simple_ko f ptr ep \<lbrace>\<lambda>_. valid_ko_at_arm\<rbrace>"
-  unfolding set_simple_ko_def set_object_def
-  apply(wpsimp wp: get_object_wp
-        simp: partial_inv_def a_type_def obj_at_def valid_ko_at_arm_def)+
-  done
-
-lemma set_thread_state_globals_equiv:
-  "\<lbrace>globals_equiv s and valid_ko_at_arm\<rbrace> set_thread_state ref ts \<lbrace>\<lambda>_. globals_equiv s\<rbrace>"
-  unfolding set_thread_state_def
-  apply(wp set_object_globals_equiv dxo_wp_weak |simp)+
-  apply (intro impI conjI allI)
-  apply(clarsimp simp: valid_ko_at_arm_def obj_at_def tcb_at_def2 get_tcb_def is_tcb_def dest: get_tcb_SomeD
-                 split: option.splits kernel_object.splits)+
-  done
-
-lemma set_bound_notification_globals_equiv:
-  "\<lbrace>globals_equiv s and valid_ko_at_arm\<rbrace> set_bound_notification ref ts \<lbrace>\<lambda>_. globals_equiv s\<rbrace>"
-  unfolding set_bound_notification_def
-  apply(wp set_object_globals_equiv dxo_wp_weak |simp)+
-  apply (intro impI conjI allI)
-  apply(clarsimp simp: valid_ko_at_arm_def obj_at_def tcb_at_def2 get_tcb_def is_tcb_def
-                 dest: get_tcb_SomeD
-                split: option.splits kernel_object.splits)+
-  done
-
-lemma set_object_valid_ko_at_arm[wp]:
-  "\<lbrace>valid_ko_at_arm and (\<lambda>s. ptr = arm_global_pd (arch_state s) \<longrightarrow>
-   a_type obj = AArch APageDirectory)\<rbrace>
-     set_object ptr obj \<lbrace>\<lambda>_. valid_ko_at_arm\<rbrace>"
-  by (wpsimp wp: set_object_wp
-           simp: a_type_def valid_ko_at_arm_def obj_at_def
-          split: kernel_object.splits arch_kernel_obj.splits if_splits)
-
-lemma valid_ko_at_arm_exst_update[simp]: "valid_ko_at_arm (trans_state f s) = valid_ko_at_arm s"
-  apply (simp add: valid_ko_at_arm_def)
-  done
-
-lemma set_thread_state_valid_ko_at_arm[wp]:
-  "\<lbrace>valid_ko_at_arm\<rbrace> set_thread_state ref ts \<lbrace>\<lambda>_. valid_ko_at_arm\<rbrace>"
-  unfolding set_thread_state_def
-  apply(wp set_object_valid_ko_at_arm dxo_wp_weak |simp)+
-  apply(fastforce simp: valid_ko_at_arm_def get_tcb_ko_at obj_at_def)
-  done
-
-lemma set_bound_notification_valid_ko_at_arm[wp]:
-  "\<lbrace>valid_ko_at_arm\<rbrace> set_bound_notification ref ts \<lbrace>\<lambda>_. valid_ko_at_arm\<rbrace>"
-  unfolding set_bound_notification_def
-  apply(wp set_object_valid_ko_at_arm dxo_wp_weak |simp)+
-  apply(fastforce simp: valid_ko_at_arm_def get_tcb_ko_at obj_at_def)
-  done
-
-crunch globals_equiv: cancel_badged_sends "globals_equiv s"
- (wp: filterM_preserved dxo_wp_weak ignore: reschedule_required tcb_sched_action)
-
-lemma thread_set_globals_equiv:
-  "(\<And>tcb. arch_tcb_context_get (tcb_arch (f tcb)) = arch_tcb_context_get (tcb_arch tcb))
-     \<Longrightarrow> \<lbrace>globals_equiv s and valid_ko_at_arm\<rbrace> thread_set f tptr \<lbrace>\<lambda>_. globals_equiv s\<rbrace>"
-  unfolding thread_set_def
-  apply(wp set_object_globals_equiv)
-  apply simp
-  apply (intro impI conjI allI)
-  apply(fastforce simp: valid_ko_at_arm_def obj_at_def get_tcb_def)+
-  apply (clarsimp simp: get_tcb_def tcb_at_def2 split: kernel_object.splits option.splits)
-  done
-
-lemma set_asid_pool_globals_equiv:
-  "\<lbrace>globals_equiv s and valid_ko_at_arm\<rbrace> set_asid_pool ptr pool \<lbrace>\<lambda>_. globals_equiv s\<rbrace>"
-  unfolding set_asid_pool_def
-  apply (wpsimp wp: set_object_globals_equiv[THEN hoare_set_object_weaken_pre]
-              simp: a_type_def)
-  apply (fastforce simp: valid_ko_at_arm_def obj_at_def)
-  done
 
 lemma idle_equiv_arch_state_update[simp]: "idle_equiv st (s\<lparr>arch_state := x\<rparr>) = idle_equiv st s"
-  apply (simp add: idle_equiv_def)
-  done
+  by (simp add: idle_equiv_def)
 
-crunch globals_equiv[wp]: invalidate_hw_asid_entry "globals_equiv s"
- (simp: globals_equiv_def)
+(* FIXME: This should either be straightforward or moved somewhere else *)
+lemma case_junk:
+  "(case rv of Inl e \<Rightarrow> True | Inr r \<Rightarrow> P r) \<longrightarrow> (case rv of Inl e \<Rightarrow> True | Inr r \<Rightarrow> R r) =
+   (case rv of Inl e \<Rightarrow> True | Inr r \<Rightarrow> P r \<longrightarrow> R r)"
+  by (case_tac rv; simp)
 
-crunch globals_equiv[wp]: invalidate_asid "globals_equiv s"
- (simp: globals_equiv_def)
-
-lemma globals_equiv_arm_next_asid_update[simp]:
-  "globals_equiv s (t\<lparr>arch_state := arch_state t\<lparr>arm_next_asid := x\<rparr>\<rparr>) = globals_equiv s t"
-  by (simp add: globals_equiv_def)
-
-lemma globals_equiv_arm_asid_map_update[simp]:
-  "globals_equiv s (t\<lparr>arch_state := arch_state t\<lparr>arm_asid_map := x\<rparr>\<rparr>) = globals_equiv s t"
-  by (simp add: globals_equiv_def)
-
-lemma globals_equiv_arm_hwasid_table_update[simp]:
-  "globals_equiv s (t\<lparr>arch_state := arch_state t\<lparr>arm_hwasid_table := x\<rparr>\<rparr>) = globals_equiv s t"
-  by (simp add: globals_equiv_def)
-
-lemma globals_equiv_arm_asid_table_update[simp]:
-  "globals_equiv s (t\<lparr>arch_state := arch_state t\<lparr>arm_asid_table := x\<rparr>\<rparr>) = globals_equiv s t"
-  by (simp add: globals_equiv_def)
-
-lemma find_free_hw_asid_globals_equiv[wp]:
-  "\<lbrace>globals_equiv s\<rbrace> find_free_hw_asid \<lbrace>\<lambda>_. globals_equiv s\<rbrace>"
-  unfolding find_free_hw_asid_def
-  apply(wp modify_wp invalidate_hw_asid_entry_globals_equiv
-          dmo_mol_globals_equiv invalidate_asid_globals_equiv
-       | wpc | simp add: invalidateLocalTLB_ASID_def)+
-  done
-
-lemma store_hw_asid_globals_equiv[wp]:
-  "\<lbrace>globals_equiv s\<rbrace> store_hw_asid asid hw_asid \<lbrace>\<lambda>_. globals_equiv s\<rbrace>"
-  unfolding store_hw_asid_def
-  apply(wp find_pd_for_asid_assert_wp | rule modify_wp, simp)+
-  apply(fastforce simp: globals_equiv_def)
-  done
-
-lemma get_hw_asid_globals_equiv[wp]:
-  "\<lbrace>globals_equiv s\<rbrace> get_hw_asid asid \<lbrace>\<lambda>_. globals_equiv s\<rbrace>"
-  unfolding get_hw_asid_def
-  apply(wp store_hw_asid_globals_equiv find_free_hw_asid_globals_equiv load_hw_asid_wp | wpc | simp)+
-  done
-
-lemma arm_context_switch_globals_equiv[wp]:
-  "\<lbrace>globals_equiv s\<rbrace> arm_context_switch pd asid \<lbrace>\<lambda>_. globals_equiv s\<rbrace>"
-  unfolding arm_context_switch_def  setHardwareASID_def
-  apply(wp dmo_mol_globals_equiv get_hw_asid_globals_equiv
-       | simp add: dmo_bind_valid set_current_pd_def writeTTBR0_def isb_def dsb_def )+
-  done
-
-lemma set_vm_root_globals_equiv[wp]:
-  "\<lbrace>globals_equiv s\<rbrace> set_vm_root tcb \<lbrace>\<lambda>_. globals_equiv s\<rbrace>"
-  apply (clarsimp simp:set_vm_root_def set_current_pd_def dsb_def
-                       isb_def writeTTBR0_def dmo_bind_valid)
-  apply(wp dmo_mol_globals_equiv arm_context_switch_globals_equiv whenE_inv
-        | wpc
-        | clarsimp simp: dmo_bind_valid isb_def dsb_def writeTTBR0_def)+
-   apply(wp hoare_vcg_all_lift | wp (once) hoare_drop_imps | clarsimp)+
-   done
-
-lemma invalidate_asid_entry_globals_equiv[wp]:
-  "\<lbrace>globals_equiv s\<rbrace> invalidate_asid_entry asid \<lbrace>\<lambda>_. globals_equiv s\<rbrace>"
-  unfolding invalidate_asid_entry_def
-  apply(wp invalidate_hw_asid_entry_globals_equiv invalidate_asid_globals_equiv load_hw_asid_wp)
-  apply(clarsimp)
-  done
-
-lemma flush_space_globals_equiv[wp]:
-  "\<lbrace>globals_equiv s\<rbrace> flush_space asid \<lbrace>\<lambda>_. globals_equiv s\<rbrace>"
-unfolding flush_space_def
-apply(wp dmo_mol_globals_equiv load_hw_asid_wp
-    | wpc
-    | simp add: invalidateLocalTLB_ASID_def cleanCaches_PoU_def dsb_def invalidate_I_PoU_def clean_D_PoU_def dmo_bind_valid)+
-done
-
-lemma delete_asid_pool_globals_equiv[wp]:
-  "\<lbrace>globals_equiv s\<rbrace> delete_asid_pool base ptr \<lbrace>\<lambda>_. globals_equiv s\<rbrace>"
-  unfolding delete_asid_pool_def
-  apply(wp set_vm_root_globals_equiv mapM_wp[OF _ subset_refl] modify_wp invalidate_asid_entry_globals_equiv flush_space_globals_equiv | simp)+
-  done
-
-crunch globals_equiv[wp]: invalidate_tlb_by_asid "globals_equiv s"
-  (simp: invalidateLocalTLB_ASID_def wp: dmo_mol_globals_equiv ignore: machine_op_lift do_machine_op)
-
-lemma set_pt_globals_equiv:
-  "\<lbrace>globals_equiv s and valid_ko_at_arm\<rbrace> set_pt ptr pt \<lbrace>\<lambda>_. globals_equiv s\<rbrace>"
-  unfolding set_pt_def
-  apply (wpsimp wp: set_object_globals_equiv[THEN hoare_set_object_weaken_pre]
-              simp: a_type_def)
-  apply (fastforce simp: valid_ko_at_arm_def obj_at_def)
-  done
-
-crunch globals_equiv: store_pte "globals_equiv s"
-
-lemma set_vm_root_for_flush_globals_equiv[wp]:
-  "\<lbrace>globals_equiv s\<rbrace> set_vm_root_for_flush pd asid \<lbrace>\<lambda>rv. globals_equiv s\<rbrace>"
-  unfolding set_vm_root_for_flush_def set_current_pd_def fun_app_def
-  apply(wp dmo_mol_globals_equiv | wpc | simp)+
-    apply(rule_tac Q="\<lambda>rv. globals_equiv s" in hoare_strengthen_post)
-     apply(wp | simp)+
-     done
-
-lemma flush_table_globals_equiv[wp]:
-  "\<lbrace>globals_equiv s\<rbrace> flush_table pd asid cptr pt \<lbrace>\<lambda>rv. globals_equiv s\<rbrace>"
-  unfolding flush_table_def invalidateLocalTLB_ASID_def fun_app_def
-  apply (wp mapM_wp' dmo_mol_globals_equiv | wpc | simp add: do_machine_op_bind split del: if_split cong: if_cong)+
-  done
-
-lemma arm_global_pd_arm_asid_map_update[simp]:
-  "arm_global_pd (arch_state s\<lparr>arm_asid_map := x\<rparr>) = arm_global_pd (arch_state s)"
-  by (simp add: globals_equiv_def)
-
-lemma arm_global_pd_arm_hwasid_table_update[simp]:
-  "arm_global_pd (arch_state s\<lparr>arm_hwasid_table := x\<rparr>) = arm_global_pd (arch_state s)"
-  by (simp add: globals_equiv_def)
-
-crunch arm_global_pd[wp]: flush_table "\<lambda>s. P (arm_global_pd (arch_state s))"
-  (wp: crunch_wps simp: crunch_simps)
-
-crunch globals_equiv[wp]: page_table_mapped "globals_equiv st"
-
-(*FIXME: duplicated, more reasonable version of not_in_global_refs_vs_lookup *)
-
-lemma not_in_global_refs_vs_lookup2: "\<lbrakk>
-  valid_vs_lookup s;
-  valid_global_refs s;
-  valid_arch_state s; valid_global_objs s; page_directory_at p s; (\<exists>\<rhd> p) s\<rbrakk> \<Longrightarrow>
-  p \<notin> global_refs s"
-  apply (insert not_in_global_refs_vs_lookup[where p=p and s=s])
-  apply simp
-done
-
-(*FIXME: This should either be straightforward or moved somewhere else*)
-
-lemma case_junk : "((case rv of Inl e \<Rightarrow> True | Inr r \<Rightarrow> P r) \<longrightarrow> (case rv of Inl e \<Rightarrow> True | Inr r \<Rightarrow> R r)) =
-  (case rv of Inl e \<Rightarrow> True | Inr r \<Rightarrow> P r \<longrightarrow> R r)"
-  apply (case_tac rv)
-  apply simp+
-done
-
-(*FIXME: Same here*)
-lemma hoare_add_postE : "\<lbrace>Q\<rbrace> f \<lbrace>\<lambda> r. P r\<rbrace>,- \<Longrightarrow> \<lbrace>Q\<rbrace> f \<lbrace>\<lambda> r s. (P r s) \<longrightarrow> (R r s) \<rbrace>,- \<Longrightarrow> \<lbrace>Q\<rbrace> f \<lbrace>\<lambda> r. R r\<rbrace>,-"
+(* FIXME: Same here *)
+lemma hoare_add_postE:
+  "\<lbrakk> \<lbrace>Q\<rbrace> f \<lbrace>P\<rbrace>, - ; \<lbrace>Q\<rbrace> f \<lbrace>\<lambda>rv s. (P rv s) \<longrightarrow> (R rv s)\<rbrace>, - \<rbrakk>
+     \<Longrightarrow> \<lbrace>Q\<rbrace> f \<lbrace>R\<rbrace>,-"
   unfolding validE_R_def validE_def
   apply (erule hoare_add_post)
    apply simp
   apply (erule hoare_post_imp[rotated])
   apply (simp add: case_junk)
-done
-
-lemma find_pd_for_asid_not_arm_global_pd:
-  "\<lbrace>pspace_aligned and valid_vspace_objs and valid_global_objs and valid_vs_lookup
-  and valid_global_refs and valid_arch_state\<rbrace>
-  find_pd_for_asid asid
-  \<lbrace>\<lambda>rv s. lookup_pd_slot rv vptr && ~~ mask pd_bits \<noteq> arm_global_pd (arch_state s)\<rbrace>, -"
-  apply (wp find_pd_for_asid_lots)
-  apply clarsimp
-  apply (subst(asm) lookup_pd_slot_pd)
-   apply (erule page_directory_at_aligned_pd_bits, simp+)
-  apply (frule (4) not_in_global_refs_vs_lookup2)
-   apply (auto simp: global_refs_def)
-done
-
-lemma find_pd_for_asid_not_arm_global_pd_large_page:
-  "\<lbrace>pspace_aligned and valid_vspace_objs and valid_global_objs and valid_vs_lookup
-  and valid_global_refs and valid_arch_state\<rbrace>
-  find_pd_for_asid asid
-  \<lbrace>\<lambda>rv s.
-  (lookup_pd_slot rv vptr && mask 6 = 0) \<longrightarrow>
-  (\<forall> x \<in> set [0 , 4 .e. 0x3C].
-  x + lookup_pd_slot rv vptr && ~~ mask pd_bits \<noteq> arm_global_pd (arch_state s))\<rbrace>, -"
-  apply (wp find_pd_for_asid_lots)
-  apply clarsimp
-  apply (subst (asm) is_aligned_mask[symmetric])
-  apply (frule is_aligned_6_masks[where bits=pd_bits])
-  apply simp+
-  apply (subst(asm) lookup_pd_slot_eq)
-   apply (erule page_directory_at_aligned_pd_bits, simp+)
-  apply (frule (4) not_in_global_refs_vs_lookup2)
-   apply (auto simp: global_refs_def)
-  done
-
-declare dmo_mol_globals_equiv[wp]
-
-lemma unmap_page_table_globals_equiv:
-  "\<lbrace>pspace_aligned and valid_vspace_objs and valid_global_objs and valid_vs_lookup
-  and valid_global_refs and valid_arch_state and globals_equiv st\<rbrace> unmap_page_table asid vaddr pt \<lbrace>\<lambda>rv. globals_equiv st\<rbrace>"
-  unfolding unmap_page_table_def page_table_mapped_def
-  apply(wp store_pde_globals_equiv | wpc | simp add: cleanByVA_PoU_def)+
-    apply(rule_tac Q="\<lambda>_. globals_equiv st and (\<lambda>sa. lookup_pd_slot pd vaddr && ~~ mask pd_bits \<noteq> arm_global_pd (arch_state sa))" in hoare_strengthen_post)
-     apply(wp find_pd_for_asid_not_arm_global_pd hoare_post_imp_dc2E_actual | simp)+
-  done
-
-lemma set_pt_valid_ko_at_arm[wp]:
-  "\<lbrace>valid_ko_at_arm\<rbrace> set_pt ptr pt \<lbrace>\<lambda>_. valid_ko_at_arm\<rbrace>"
-  unfolding set_pt_def
-  by (wpsimp wp: set_object_wp_strong simp: valid_ko_at_arm_def obj_at_def a_type_def)
-
-crunch valid_ko_at_arm[wp]: store_pte "valid_ko_at_arm"
-
-lemma mapM_x_swp_store_pte_globals_equiv:
-  " \<lbrace>globals_equiv s and valid_ko_at_arm\<rbrace>
-          mapM_x (swp store_pte A) slots
-          \<lbrace>\<lambda>_. globals_equiv s\<rbrace>"
-  apply(rule_tac Q="\<lambda>_. globals_equiv s and valid_ko_at_arm" in hoare_strengthen_post)
-   apply(wp mapM_x_wp' store_pte_globals_equiv store_pte_valid_ko_at_arm | simp)+
-   done
-
-lemma mapM_x_swp_store_pte_valid_ko_at_arm[wp]:
-  " \<lbrace>valid_ko_at_arm\<rbrace>
-          mapM_x (swp store_pte A) slots
-          \<lbrace>\<lambda>_. valid_ko_at_arm\<rbrace>"
-  apply(wp mapM_x_wp' | simp add: swp_def)+
-  done
-
-lemma set_cap_globals_equiv'':
-  "\<lbrace>globals_equiv s and valid_ko_at_arm\<rbrace>
-  set_cap cap p \<lbrace>\<lambda>_. globals_equiv s\<rbrace>"
-  unfolding set_cap_def
-  apply(simp only: split_def)
-  apply(wp set_object_globals_equiv hoare_vcg_all_lift get_object_wp | wpc | simp)+
-   apply(fastforce simp: valid_ko_at_arm_def valid_ao_at_def obj_at_def is_tcb_def)+
-  done
-
-lemma do_machine_op_valid_ko_at_arm[wp]:
-  "\<lbrace>valid_ko_at_arm\<rbrace> do_machine_op mol \<lbrace>\<lambda>_. valid_ko_at_arm\<rbrace>"
-  unfolding do_machine_op_def machine_op_lift_def split_def valid_ko_at_arm_def
-  apply(wp modify_wp, simp)
-  done
-
-lemma valid_ko_at_arm_next_asid[simp]:
-  "valid_ko_at_arm (s\<lparr>arch_state := arch_state s\<lparr>arm_next_asid := x\<rparr>\<rparr>)
-  = valid_ko_at_arm s"
-  by (simp add: valid_ko_at_arm_def)
-
-lemma valid_ko_at_arm_asid_map[simp]:
-  "valid_ko_at_arm (s\<lparr>arch_state := arch_state s\<lparr>arm_asid_map := x\<rparr>\<rparr>)
-  = valid_ko_at_arm s"
-  by (simp add: valid_ko_at_arm_def)
-
-lemma valid_ko_at_arm_hwasid_table[simp]:
-  "valid_ko_at_arm (s\<lparr>arch_state := arch_state s\<lparr>arm_hwasid_table := x\<rparr>\<rparr>)
-  = valid_ko_at_arm s"
-  by (simp add: valid_ko_at_arm_def)
-
-lemma valid_ko_at_arm_asid_table[simp]:
-  "valid_ko_at_arm
-                (s\<lparr>arch_state := arch_state s
-                     \<lparr>arm_asid_table := A\<rparr>\<rparr>) =
-   valid_ko_at_arm s" by (simp add: valid_ko_at_arm_def)
-
-lemma valid_ko_at_arm_interrupt_states[simp]:
-  "valid_ko_at_arm (s\<lparr>interrupt_states := f\<rparr>)
-  = valid_ko_at_arm s"
-  by (simp add: valid_ko_at_arm_def)
-
-lemma valid_ko_at_arm_arch[simp]:
-  "arm_global_pd A = arm_global_pd (arch_state s) \<Longrightarrow>
-   valid_ko_at_arm (s\<lparr>arch_state := A\<rparr>) = valid_ko_at_arm s"
-  by (simp add: valid_ko_at_arm_def)
-
-crunch valid_ko_at_arm[wp]: arm_context_switch, set_vm_root, set_pd "valid_ko_at_arm"
-  (wp: find_pd_for_asid_assert_wp crunch_wps simp: crunch_simps)
-
-crunch valid_ko_at_arm[wp]: unmap_page_table "valid_ko_at_arm"
-  (wp: crunch_wps simp: crunch_simps a_type_simps)
-
-definition authorised_for_globals_page_table_inv ::
-    "page_table_invocation \<Rightarrow> 'z state \<Rightarrow> bool" where
-  "authorised_for_globals_page_table_inv pti \<equiv>
-    \<lambda>s. case pti of PageTableMap cap ptr pde p
-  \<Rightarrow> p && ~~ mask pd_bits \<noteq> arm_global_pd (arch_state s) | _ \<Rightarrow> True"
-
-lemma perform_page_table_invocation_globals_equiv:
-  "\<lbrace>valid_global_refs and valid_global_objs and valid_arch_state and
-    globals_equiv st and pspace_aligned and valid_vspace_objs and
-    valid_vs_lookup and valid_kernel_mappings and authorised_for_globals_page_table_inv pti\<rbrace>
-  perform_page_table_invocation pti \<lbrace>\<lambda>_. globals_equiv st\<rbrace>"
-  unfolding perform_page_table_invocation_def cleanCacheRange_PoU_def
-  apply(rule hoare_weaken_pre)
-   apply(wp store_pde_globals_equiv set_cap_globals_equiv'' dmo_cacheRangeOp_lift
-            mapM_x_swp_store_pte_globals_equiv unmap_page_table_globals_equiv
-           | wpc | simp add: cleanByVA_PoU_def)+
-  apply(fastforce simp: authorised_for_globals_page_table_inv_def valid_arch_state_def valid_ko_at_arm_def obj_at_def dest: a_type_pdD)
-  done
-
-lemma do_flush_globals_equiv:
-  "\<lbrace>globals_equiv st\<rbrace> do_machine_op (do_flush typ start end pstart)
-    \<lbrace>\<lambda>rv. globals_equiv st\<rbrace>"
-  apply (cases "typ")
-     apply (wp dmo_cacheRangeOp_lift | simp add: do_flush_def cache_machine_op_defs do_flush_defs do_machine_op_bind when_def | clarsimp | rule conjI)+
-     done
-
-lemma perform_page_directory_invocation_globals_equiv:
-  "\<lbrace>globals_equiv st\<rbrace>
-  perform_page_directory_invocation pdi \<lbrace>\<lambda>_. globals_equiv st\<rbrace>"
-  unfolding perform_page_directory_invocation_def
-  apply (cases pdi)
-   apply (wp do_flush_globals_equiv | simp)+
-   done
-
-lemma flush_page_globals_equiv[wp]:
-  "\<lbrace>globals_equiv st\<rbrace> flush_page page_size pd asid vptr \<lbrace>\<lambda>_. globals_equiv st\<rbrace>"
-  unfolding flush_page_def invalidateLocalTLB_VAASID_def
-  apply(wp | simp cong: if_cong split del: if_split)+
-  done
-
-lemma flush_page_arm_global_pd[wp]:
-  "\<lbrace>\<lambda>s. P (arm_global_pd (arch_state s))\<rbrace>
-     flush_page pgsz pd asid vptr
-   \<lbrace>\<lambda>rv s. P (arm_global_pd (arch_state s))\<rbrace>"
-  unfolding flush_page_def
-  apply(wp | simp cong: if_cong split del: if_split)+
-  done
-
-lemma mapM_swp_store_pte_globals_equiv:
-  "\<lbrace>globals_equiv st and valid_ko_at_arm\<rbrace>
-    mapM (swp store_pte A) slots \<lbrace>\<lambda>_. globals_equiv st\<rbrace>"
-  apply(rule_tac Q="\<lambda> _. globals_equiv st and valid_ko_at_arm"
-        in hoare_strengthen_post)
-   apply(wp mapM_wp' store_pte_globals_equiv | simp)+
-   done
-
-lemma mapM_swp_store_pde_globals_equiv:
-  "\<lbrace>globals_equiv st and (\<lambda>s. \<forall>x \<in> set slots.
-   x && ~~ mask pd_bits \<noteq> arm_global_pd (arch_state s))\<rbrace>
-     mapM (swp store_pde A) slots \<lbrace>\<lambda>_. globals_equiv st\<rbrace>"
-  apply (rule_tac Q="\<lambda> _. globals_equiv st and (\<lambda> s. \<forall>x \<in> set slots.
-                      x && ~~ mask pd_bits \<noteq> arm_global_pd (arch_state s))"
-         in hoare_strengthen_post)
-   apply (wp mapM_wp' store_pde_globals_equiv | simp)+
-   done
-
-lemma mapM_swp_store_pte_valid_ko_at_arm[wp]:
-  "\<lbrace>valid_ko_at_arm\<rbrace> mapM (swp store_pte A) slots \<lbrace>\<lambda>_. valid_ko_at_arm\<rbrace>"
-  apply(wp mapM_wp' store_pte_valid_ko_at_arm | simp)+
-  done
-
-lemma mapM_x_swp_store_pde_globals_equiv :
-  "\<lbrace>globals_equiv st and (\<lambda>s. \<forall>x \<in> set slots.
-   x && ~~ mask pd_bits \<noteq> arm_global_pd (arch_state s))\<rbrace>
-     mapM_x (swp store_pde A) slots \<lbrace>\<lambda>_. globals_equiv st\<rbrace>"
-  apply (rule_tac Q="\<lambda>_. globals_equiv st and (\<lambda> s. \<forall>x \<in> set slots.
-                     x && ~~ mask pd_bits \<noteq> arm_global_pd (arch_state s))"
-         in hoare_strengthen_post)
-   apply (wp mapM_x_wp' store_pde_globals_equiv | simp)+
-   done
-
-crunch valid_ko_at_arm[wp]: flush_page "valid_ko_at_arm"
-  (wp: crunch_wps simp: crunch_simps)
-
-lemma unmap_page_globals_equiv:
-  "\<lbrace>globals_equiv st and valid_arch_state and pspace_aligned and valid_vspace_objs
-  and valid_global_objs and valid_vs_lookup and valid_global_refs \<rbrace> unmap_page pgsz asid vptr pptr
-   \<lbrace>\<lambda>_. globals_equiv st\<rbrace>"
-  unfolding unmap_page_def cleanCacheRange_PoU_def including no_pre
-  apply (induct pgsz)
-     prefer 4
-     apply (simp only: vmpage_size.simps)
-     apply(wp mapM_swp_store_pde_globals_equiv dmo_cacheRangeOp_lift | simp add: cleanByVA_PoU_def)+
-        apply(rule hoare_drop_imps)
-        apply(wp)+
-       apply(simp)
-       apply(rule hoare_drop_imps)
-       apply(wp)+
-     apply (rule hoare_pre)
-      apply (rule_tac Q="\<lambda>x. globals_equiv st and (\<lambda>sa. lookup_pd_slot x vptr && mask 6 = 0 \<longrightarrow> (\<forall>xa\<in>set [0 , 4 .e. 0x3C]. xa + lookup_pd_slot x vptr && ~~ mask pd_bits \<noteq> arm_global_pd (arch_state sa)))" and E="\<lambda>_. globals_equiv st" in hoare_post_impErr)
-        apply(wp find_pd_for_asid_not_arm_global_pd_large_page)
-       apply simp
-      apply simp
-     apply simp
-    apply(wp store_pte_globals_equiv | simp add: cleanByVA_PoU_def)+
-      apply(wp hoare_drop_imps)+
-     apply(wp (once) lookup_pt_slot_inv)
-     apply(wp (once) lookup_pt_slot_inv)
-     apply(wp (once) lookup_pt_slot_inv)
-     apply(wp (once) lookup_pt_slot_inv)
-    apply(simp)
-    apply(rule hoare_pre)
-     apply wp
-    apply(simp add: valid_arch_state_ko_at_arm)
-   apply(simp)
-   apply(rule hoare_pre)
-    apply(wp dmo_cacheRangeOp_lift mapM_swp_store_pde_globals_equiv store_pde_globals_equiv lookup_pt_slot_inv mapM_swp_store_pte_globals_equiv hoare_drop_imps | simp add: cleanByVA_PoU_def)+
-   apply(simp add: valid_arch_state_ko_at_arm)
-  apply(rule hoare_pre)
-   apply(wp store_pde_globals_equiv | simp add: valid_arch_state_ko_at_arm cleanByVA_PoU_def)+
-    apply(wp find_pd_for_asid_not_arm_global_pd hoare_drop_imps)+
-  apply(clarsimp)
-  done (* don't know what happened here. wp deleted globals_equiv from precon *)
-
-
-lemma cte_wp_parent_not_global_pd: "valid_global_refs s \<Longrightarrow> cte_wp_at (parent_for_refs (Inr (a,b))) k s \<Longrightarrow> \<forall>x \<in> set b. x && ~~ mask pd_bits \<noteq> arm_global_pd (arch_state s)"
-  apply (simp only: cte_wp_at_caps_of_state)
-  apply (elim exE conjE)
-  apply (drule valid_global_refsD2,simp)
-  apply (unfold parent_for_refs_def)
-  apply (simp add: image_def global_refs_def cap_range_def)
-  apply clarsimp
-  apply (subgoal_tac "arm_global_pd (arch_state s) \<in> set b")
-   apply auto
-  done
-
-definition authorised_for_globals_page_inv :: "page_invocation \<Rightarrow> 'z::state_ext state \<Rightarrow> bool"
-  where "authorised_for_globals_page_inv pgi \<equiv>
-    \<lambda>s. case pgi of PageMap asid cap ptr m \<Rightarrow> \<exists>slot. cte_wp_at (parent_for_refs m) slot s | _ \<Rightarrow> True"
-
-lemma set_cap_valid_ko_at_arm[wp]:
-  "\<lbrace>valid_ko_at_arm\<rbrace> set_cap cap p \<lbrace>\<lambda>_. valid_ko_at_arm\<rbrace>"
-  apply(simp add: valid_ko_at_arm_def)
-  apply(rule hoare_ex_wp)
-  apply(rule hoare_pre)
-   apply(simp add: set_cap_def split_def)
-   apply(wp | wpc)+
-     apply(simp add: set_object_def)
-     apply(wp get_object_wp | wpc)+
-  apply(fastforce simp: obj_at_def)
-  done
-
-crunch valid_ko_at_arm[wp]: unmap_page "valid_ko_at_arm"
-  (wp: crunch_wps)
-
-lemma as_user_globals_equiv:
-  "\<lbrace>globals_equiv s and valid_ko_at_arm and (\<lambda>s. tptr \<noteq> idle_thread s)\<rbrace> as_user tptr f
-    \<lbrace>\<lambda>_. globals_equiv s\<rbrace>"
-  unfolding as_user_def
-  apply(wp)
-      apply(simp add: split_def)
-      apply(wp set_object_globals_equiv)+
-  apply(clarsimp simp: valid_ko_at_arm_def get_tcb_def obj_at_def)
-  done
-
-
-lemma set_message_info_globals_equiv:
-  "\<lbrace>globals_equiv s and valid_ko_at_arm and (\<lambda>s. thread \<noteq> idle_thread s)\<rbrace> set_message_info thread info \<lbrace>\<lambda>_. globals_equiv s\<rbrace>"
-  unfolding set_message_info_def
-  apply(wp as_user_globals_equiv)
   done
 
 lemma store_word_offs_globals_equiv:
-  "\<lbrace>globals_equiv s\<rbrace>
-    store_word_offs ptr offs v
-    \<lbrace>\<lambda>_. globals_equiv s\<rbrace>"
+  "store_word_offs ptr offs v \<lbrace>globals_equiv s\<rbrace>"
   unfolding store_word_offs_def fun_app_def
   apply (wp do_machine_op_globals_equiv)
-    apply clarsimp
-    apply (erule use_valid[OF _ storeWord_globals_equiv])
-    apply (wp | simp | force)+
+     apply clarsimp
+     apply (erule use_valid[OF _ storeWord_globals_equiv])
+     apply (wp | simp | force)+
   done
-
-
-lemma length_msg_registers:
-  "length msg_registers = 4"
-  unfolding msg_registers_def
-  by (simp add: msgRegisters_def upto_enum_def fromEnum_def enum_register)
-
-lemma length_msg_lt_msg_max:
-  "length msg_registers < msg_max_length"
-  apply(simp add: length_msg_registers msg_max_length_def)
-  done
-
-
-lemma arm_global_pd_not_tcb:
-  "valid_ko_at_arm s \<Longrightarrow> get_tcb (arm_global_pd (arch_state s)) s = None"
-  unfolding valid_ko_at_arm_def
-  apply (case_tac "get_tcb (arm_global_pd (arch_state s)) s")
-  apply simp
-  apply(clarsimp simp: valid_ko_at_arm_def get_tcb_ko_at obj_at_def)
-  done
-
-
-lemma set_mrs_globals_equiv:
-  "\<lbrace>globals_equiv s and valid_ko_at_arm and (\<lambda>sa. thread \<noteq> idle_thread sa)\<rbrace>
-      set_mrs thread buf msgs
-    \<lbrace>\<lambda>_. globals_equiv s\<rbrace>"
-  unfolding set_mrs_def
-  apply(wp | wpc)+
-       apply(simp add: zipWithM_x_mapM_x)
-       apply(rule conjI)
-        apply(rule impI)
-        apply(rule_tac Q="\<lambda>_. globals_equiv s"
-          in hoare_strengthen_post)
-         apply(wp mapM_x_wp')
-         apply(simp add: split_def)
-         apply(wp store_word_offs_globals_equiv)
-        apply(simp)
-       apply(clarsimp)
-       apply(insert length_msg_lt_msg_max)
-       apply(simp)
-      apply(wp set_object_globals_equiv static_imp_wp)
-     apply(wp hoare_vcg_all_lift set_object_globals_equiv static_imp_wp)+
-   apply(clarsimp simp:arm_global_pd_not_tcb)+
-  done
-
-crunch valid_ko_at_arm[wp]: set_mrs valid_ko_at_arm
-  (wp: crunch_wps simp: crunch_simps arm_global_pd_not_tcb)
-
-lemma perform_page_invocation_globals_equiv:
-  "\<lbrace>authorised_for_globals_page_inv pgi and valid_page_inv pgi and globals_equiv st
-    and valid_arch_state and pspace_aligned and valid_vspace_objs and valid_global_objs
-    and valid_vs_lookup and valid_global_refs and ct_active and valid_idle\<rbrace>
-   perform_page_invocation pgi
-   \<lbrace>\<lambda>_. globals_equiv st\<rbrace>"
-  unfolding perform_page_invocation_def cleanCacheRange_PoU_def
-  apply(rule hoare_weaken_pre)
-  apply(wp mapM_swp_store_pte_globals_equiv hoare_vcg_all_lift dmo_cacheRangeOp_lift
-        mapM_swp_store_pde_globals_equiv mapM_x_swp_store_pte_globals_equiv
-        mapM_x_swp_store_pde_globals_equiv set_cap_globals_equiv''
-        unmap_page_globals_equiv store_pte_globals_equiv store_pde_globals_equiv static_imp_wp
-        do_flush_globals_equiv set_mrs_globals_equiv set_message_info_globals_equiv
-       | wpc | simp add: do_machine_op_bind cleanByVA_PoU_def)+
-  by (auto simp: cte_wp_parent_not_global_pd authorised_for_globals_page_inv_def
-                   valid_page_inv_def valid_slots_def valid_idle_def st_tcb_def2 ct_in_state_def
-                   pred_tcb_at_def obj_at_def
-           dest: valid_arch_state_ko_at_arm
-           dest!:rev_subsetD[OF _ tl_subseteq])
-
-lemma retype_region_ASIDPoolObj_globals_equiv:
-  "\<lbrace>globals_equiv s and (\<lambda>sa. ptr \<noteq> arm_global_pd (arch_state s)) and (\<lambda>sa. ptr \<noteq> idle_thread sa)\<rbrace>
-  retype_region ptr 1 0 (ArchObject ASIDPoolObj) dev
-  \<lbrace>\<lambda>_. globals_equiv s\<rbrace>"
-  unfolding retype_region_def
-  apply(wp modify_wp dxo_wp_weak | simp | fastforce simp: globals_equiv_def default_arch_object_def obj_bits_api_def)+
-      apply (simp add: trans_state_update[symmetric] del: trans_state_update)
-     apply wp+
-  apply (fastforce simp: globals_equiv_def idle_equiv_def tcb_at_def2)
-  done
-
-crunch valid_ko_at_arm[wp]: "set_untyped_cap_as_full" "valid_ko_at_arm"
-
-lemma cap_insert_globals_equiv'':
-  "\<lbrace>globals_equiv s and valid_global_objs and valid_ko_at_arm\<rbrace>
-  cap_insert new_cap src_slot dest_slot \<lbrace>\<lambda>_. globals_equiv s\<rbrace>"
-  unfolding  cap_insert_def
-  apply(wp set_original_globals_equiv update_cdt_globals_equiv set_cap_globals_equiv'' dxo_wp_weak
-         | rule hoare_drop_imps | simp)+
-  done
-
-
-
-lemma retype_region_ASIDPoolObj_valid_ko_at_arm:
-  "\<lbrace>valid_ko_at_arm and (\<lambda>s. ptr \<noteq> arm_global_pd (arch_state s))\<rbrace>
-  retype_region ptr 1 0 (ArchObject ASIDPoolObj) dev
-  \<lbrace>\<lambda>_. valid_ko_at_arm\<rbrace>"
-  apply(simp add: retype_region_def)
-  apply(wp modify_wp dxo_wp_weak |simp add: trans_state_update[symmetric] del: trans_state_update)+
-  apply(clarsimp simp: valid_ko_at_arm_def)
-  apply(rule_tac x=pd in exI)
-  apply(fold fun_upd_def)
-  apply(clarsimp simp: fun_upd_def obj_at_def)
-  done
-
-lemma detype_valid_ko_at_arm:
-  "\<lbrace>valid_ko_at_arm and (\<lambda>s.
-      arm_global_pd (arch_state s) \<notin> {ptr..ptr + 2 ^ bits - 1})\<rbrace>
-   modify (detype {ptr..ptr + 2 ^ bits - 1}) \<lbrace>\<lambda>_. valid_ko_at_arm\<rbrace>"
-  apply(wp modify_wp)
-  apply(fastforce simp: valid_ko_at_arm_def detype_def obj_at_def)
-  done
-
-lemma detype_valid_arch_state:
-  "\<lbrace>valid_arch_state and
-    (\<lambda>s. arm_globals_frame (arch_state s) \<notin> {ptr..ptr + 2 ^ bits - 1} \<and>
-         arm_global_pd (arch_state s) \<notin> {ptr..ptr + 2 ^ bits - 1} \<and>
-    {ptr..ptr + 2 ^ bits - 1} \<inter> ran (arm_asid_table (arch_state s)) = {} \<and>
-    {ptr..ptr + 2 ^ bits - 1} \<inter> set (arm_global_pts (arch_state s)) = {})\<rbrace>
-   modify (detype {ptr..ptr + (1 << bits) - 1}) \<lbrace>\<lambda>_. valid_arch_state\<rbrace>"
-  apply(wp modify_wp)
-  apply(simp add: valid_arch_state_def)
-  apply(rule conjI)
-   apply(clarsimp simp: valid_asid_table_def)
-   apply(erule_tac x=p in in_empty_interE)
-    apply(simp)+
-  apply(clarsimp simp: valid_global_pts_def)
-  apply(erule_tac x=p and B="set (arm_global_pts (arch_state s))" in in_empty_interE)
-   apply(simp)+
-   done
-
-
-lemma delete_objects_valid_ko_at_arm:
-   "\<lbrace>valid_ko_at_arm and
-   (\<lambda>s. arm_global_pd (arch_state s) \<notin> ptr_range p b) and
-    K (is_aligned p b \<and>
-        2 \<le> b \<and>
-        b < word_bits)\<rbrace>
-  delete_objects p b \<lbrace>\<lambda>_. valid_ko_at_arm\<rbrace>"
-  apply(rule hoare_gen_asm)
-  unfolding delete_objects_def
-  apply(wp detype_valid_ko_at_arm do_machine_op_valid_ko_at_arm | simp add: ptr_range_def)+
-  done
-
-lemma perform_asid_control_invocation_globals_equiv:
-  notes delete_objects_invs[wp del]
-  notes blah[simp del] =  atLeastAtMost_iff atLeastatMost_subset_iff atLeastLessThan_iff
-  shows
-  "\<lbrace>globals_equiv s and invs and ct_active and valid_aci aci\<rbrace>
-   perform_asid_control_invocation aci \<lbrace>\<lambda>_. globals_equiv s\<rbrace>"
-  unfolding perform_asid_control_invocation_def
-  apply(rule hoare_pre)
-   apply wpc
-   apply (rename_tac word1 cslot_ptr1 cslot_ptr2 word2)
-   apply (wp modify_wp cap_insert_globals_equiv''
-             retype_region_ASIDPoolObj_globals_equiv[simplified]
-             retype_region_invs_extras(5)[where sz=pageBits]
-             retype_region_ASIDPoolObj_valid_ko_at_arm[simplified]
-             set_cap_globals_equiv
-             max_index_upd_invs_simple set_cap_no_overlap
-             set_cap_caps_no_overlap max_index_upd_caps_overlap_reserved
-             region_in_kernel_window_preserved
-             hoare_vcg_all_lift  get_cap_wp static_imp_wp
-             set_cap_idx_up_aligned_area[where dev = False,simplified]
-         | simp)+
-   (* factor out the implication -- we know what the relevant components of the
-      cap referred to in the cte_wp_at are anyway from valid_aci, so just use
-      those directly to simplify the reasoning later on *)
-   apply(rule_tac Q="\<lambda> a b. globals_equiv s b \<and>
-                            invs b \<and> valid_ko_at_arm b \<and> word1 \<noteq> arm_global_pd (arch_state b) \<and>
-                            word1 \<noteq> idle_thread b \<and>
-                            (\<exists> idx. cte_wp_at ((=) (UntypedCap False word1 pageBits idx)) cslot_ptr2 b) \<and>
-                             descendants_of cslot_ptr2 (cdt b) = {} \<and>
-                             pspace_no_overlap_range_cover word1 pageBits b"
-         in hoare_strengthen_post)
-    prefer 2
-    apply (clarsimp simp: globals_equiv_def invs_valid_global_objs)
-    apply (drule cte_wp_at_eqD2, assumption)
-    apply clarsimp
-    apply (clarsimp simp: empty_descendants_range_in)
-    apply (rule conjI, fastforce simp: cte_wp_at_def)
-    apply (clarsimp simp: obj_bits_api_def default_arch_object_def)
-    apply (frule untyped_cap_aligned, simp add: invs_valid_objs)
-    apply (clarsimp simp: cte_wp_at_caps_of_state)
-    apply (strengthen refl caps_region_kernel_window_imp[mk_strg I E])
-    apply (simp add: invs_valid_objs invs_cap_refs_in_kernel_window
-                     atLeastatMost_subset_iff word_and_le2)
-    apply(rule conjI, rule descendants_range_caps_no_overlapI)
-       apply assumption
-      apply(simp add: cte_wp_at_caps_of_state)
-     apply(simp add: empty_descendants_range_in)
-    apply(clarsimp simp: range_cover_def)
-    apply(subst is_aligned_neg_mask_eq[THEN sym], assumption)
-    apply(simp add: word_bw_assocs pageBits_def mask_zero)
-   apply(wp add: delete_objects_invs_ex delete_objects_pspace_no_overlap[where dev=False]
-            delete_objects_globals_equiv delete_objects_valid_ko_at_arm
-            hoare_vcg_ex_lift
-            del: Untyped_AI.delete_objects_pspace_no_overlap
-        | simp add: page_bits_def)+
-  apply (clarsimp simp: conj_comms invs_valid_ko_at_arm invs_psp_aligned invs_valid_objs valid_aci_def)
-  apply (clarsimp simp: cte_wp_at_caps_of_state)
-  apply (frule_tac cap="UntypedCap False a b c" for a b c  in caps_of_state_valid, assumption)
-  apply (clarsimp simp: valid_cap_def cap_aligned_def untyped_min_bits_def)
-  apply (frule_tac slot="(aa,ba)" in untyped_caps_do_not_overlap_global_refs[rotated, OF invs_valid_global_refs])
-   apply (clarsimp simp: cte_wp_at_caps_of_state)
-   apply ((rule conjI |rule refl | simp)+)[1]
-  apply(rule conjI)
-   apply(clarsimp simp: global_refs_def ptr_range_memI)
-  apply(rule conjI)
-   apply(clarsimp simp: global_refs_def ptr_range_memI)
-  apply(rule conjI, fastforce simp: global_refs_def)
-  apply(rule conjI, fastforce simp: global_refs_def)
-  apply(rule conjI)
-   apply(drule untyped_slots_not_in_untyped_range)
-        apply(blast intro!: empty_descendants_range_in)
-       apply(simp add: cte_wp_at_caps_of_state)
-      apply simp
-     apply(rule refl)
-    apply(rule subset_refl)
-   apply(simp)
-  apply(rule conjI)
-   apply fastforce
-  apply (auto intro: empty_descendants_range_in simp: descendants_range_def2 cap_range_def)
-  done
-
-
-lemma perform_asid_pool_invocation_globals_equiv:
-  "\<lbrace>globals_equiv s and valid_ko_at_arm\<rbrace> perform_asid_pool_invocation api \<lbrace>\<lambda>_. globals_equiv s\<rbrace>"
-  unfolding perform_asid_pool_invocation_def
-  apply(rule hoare_weaken_pre)
-   apply(wp modify_wp set_asid_pool_globals_equiv set_cap_globals_equiv''
-        get_cap_wp | wpc | simp)+
-  done
-
-definition
-  authorised_for_globals_arch_inv :: "arch_invocation \<Rightarrow> ('z::state_ext) state \<Rightarrow> bool" where
-  "authorised_for_globals_arch_inv ai \<equiv> case ai of
-  InvokePageTable oper \<Rightarrow> authorised_for_globals_page_table_inv oper |
-  InvokePage oper \<Rightarrow> authorised_for_globals_page_inv oper |
-  _ \<Rightarrow> \<top>"
-
-lemma arch_perform_invocation_globals_equiv:
-  "\<lbrace>globals_equiv s and invs and ct_active and valid_arch_inv ai and authorised_for_globals_arch_inv ai\<rbrace>
-  arch_perform_invocation ai \<lbrace>\<lambda>_. globals_equiv s\<rbrace>"
-  unfolding arch_perform_invocation_def
-  apply wp
-   apply(wpc)
-       apply(wp perform_page_table_invocation_globals_equiv perform_page_directory_invocation_globals_equiv
-                perform_page_invocation_globals_equiv perform_asid_control_invocation_globals_equiv
-                perform_asid_pool_invocation_globals_equiv)+
-  apply(auto simp: authorised_for_globals_arch_inv_def
-             dest: valid_arch_state_ko_at_arm
-             simp: invs_def valid_state_def valid_arch_inv_def invs_valid_vs_lookup)
-  done
-
-lemma find_pd_for_asid_authority3:
-  "\<lbrace>\<lambda>s. \<forall>pd. (pspace_aligned s \<and> valid_vspace_objs s \<longrightarrow> is_aligned pd pd_bits)
-           \<and> (\<exists>\<rhd> pd) s
-           \<longrightarrow> Q pd s\<rbrace> find_pd_for_asid asid \<lbrace>Q\<rbrace>, -"
-  (is "\<lbrace>?P\<rbrace> ?f \<lbrace>Q\<rbrace>,-")
-  apply (clarsimp simp: validE_R_def validE_def valid_def imp_conjL[symmetric])
-  apply (frule in_inv_by_hoareD[OF find_pd_for_asid_inv], clarsimp)
-  apply (drule spec, erule mp)
-  apply (simp add: use_validE_R[OF _ find_pd_for_asid_authority1]
-                   use_validE_R[OF _ find_pd_for_asid_aligned_pd_bits]
-                   use_validE_R[OF _ find_pd_for_asid_lookup])
-  done
-
-lemma decode_arch_invocation_authorised_for_globals:
-  "\<lbrace>invs and cte_wp_at ((=) (cap.ArchObjectCap cap)) slot
-        and (\<lambda>s. \<forall>(cap, slot) \<in> set excaps. cte_wp_at ((=) cap) slot s)\<rbrace>
-  arch_decode_invocation label msg x_slot slot cap excaps
-  \<lbrace>\<lambda>rv. authorised_for_globals_arch_inv rv\<rbrace>, -"
-  unfolding arch_decode_invocation_def authorised_for_globals_arch_inv_def
-  apply (rule hoare_pre)
-   apply (simp add: split_def Let_def
-               cong: cap.case_cong arch_cap.case_cong if_cong option.case_cong
-               split del: if_split)
-   apply (wp select_wp select_ext_weak_wp whenE_throwError_wp check_vp_wpR unlessE_wp get_pde_wp get_master_pde_wp
-             find_pd_for_asid_authority3 create_mapping_entries_parent_for_refs
-           | wpc
-           | simp add:  authorised_for_globals_page_inv_def
-                  del: hoare_True_E_R
-                  split del: if_split)+
-     apply(simp cong: if_cong)
-     apply(wp hoare_vcg_if_lift2)
-     apply(rule hoare_conjI)
-      apply(rule hoare_drop_imps)
-      apply(simp add: authorised_for_globals_page_table_inv_def)
-      apply(wp)
-     apply(rule hoare_drop_imps)
-     apply((wp hoare_TrueI hoare_vcg_all_lift hoare_drop_imps | wpc | simp)+)[3]
-  apply (clarsimp simp: authorised_asid_pool_inv_def authorised_page_table_inv_def
-                        neq_Nil_conv invs_psp_aligned invs_vspace_objs cli_no_irqs)
-  apply (drule cte_wp_valid_cap, clarsimp+)
-  apply (cases cap, simp_all)
-    \<comment> \<open>PageCap\<close>
-    apply (clarsimp simp: valid_cap_simps cli_no_irqs)
-    apply (cases "invocation_type label";(rename_tac arch, case_tac arch; simp add: isPageFlushLabel_def isPDFlushLabel_def))
-           \<comment> \<open>Map\<close>
-           apply (rename_tac word cap_rights vmpage_size option arch)
-           apply(clarsimp simp: isPageFlushLabel_def isPDFlushLabel_def | rule conjI)+
-            apply(drule cte_wp_valid_cap)
-             apply(clarsimp simp: invs_def valid_state_def)
-            apply(simp add: valid_cap_def)
-           apply(simp add: vmsz_aligned_def)
-           apply(drule_tac ptr="msg ! 0" and off="2 ^ pageBitsForSize vmpage_size - 1" in is_aligned_no_wrap')
-            apply(insert pbfs_less_wb')
-            apply(clarsimp)
-           apply(fastforce simp: x_power_minus_1)
-          apply(clarsimp)
-          apply(fastforce dest: cte_wp_valid_cap simp: invs_def valid_state_def valid_cap_def)
-         \<comment> \<open>Unmap\<close>
-         apply(simp add: authorised_for_globals_page_inv_def)+
-   apply(clarsimp)
-   \<comment> \<open>PageTableCap\<close>
-   apply(simp add: authorised_for_globals_page_table_inv_def)
-   apply(clarsimp)
-   apply(frule_tac vptr="msg ! 0" in pd_shifting')
-   apply(clarsimp)
-   apply(clarsimp simp: invs_def valid_state_def valid_global_refs_def valid_refs_def global_refs_def)
-   apply(erule_tac x=aa in allE)
-   apply(erule_tac x=b in allE)
-   apply(drule_tac P'="\<lambda>c. idle_thread s \<in> cap_range c \<or>
-                 arm_global_pd (arch_state s) \<in> cap_range c \<or>
-                 (range (interrupt_irq_node s) \<union>
-                  set (arm_global_pts (arch_state s))) \<inter>
-                 cap_range c \<noteq>
-                 {}" in cte_wp_at_weakenE)
-    apply(clarsimp simp: cap_range_def)
-   apply(simp)
-  by(fastforce)
-
-
-lemma as_user_valid_ko_at_arm[wp]:
-  "\<lbrace> valid_ko_at_arm \<rbrace>
-  as_user thread f
-  \<lbrace> \<lambda>_. valid_ko_at_arm\<rbrace>"
-  unfolding as_user_def
-  apply wp
-     apply (case_tac x)
-     apply (simp | wp select_wp)+
-  apply(fastforce simp: valid_ko_at_arm_def get_tcb_ko_at obj_at_def)
-  done
-
-lemma valid_arch_arm_asid_table_unmap:
-  "valid_arch_state s
-       \<and> tab = arm_asid_table (arch_state s)
-     \<longrightarrow> valid_arch_state (s\<lparr>arch_state := arch_state s\<lparr>arm_asid_table := tab(asid_high_bits_of base := None)\<rparr>\<rparr>)"
-  apply (clarsimp simp: valid_state_def valid_arch_state_unmap_strg)
-  done
-
-lemma valid_arch_objs_arm_asid_table_unmap:
-  "valid_vspace_objs s
-       \<and> tab = arm_asid_table (arch_state s)
-     \<longrightarrow> valid_vspace_objs (s\<lparr>arch_state := arch_state s\<lparr>arm_asid_table := tab(asid_high_bits_of base := None)\<rparr>\<rparr>)"
-  apply (clarsimp simp: valid_state_def valid_vspace_objs_unmap_strg)
-  done
-
-lemma valid_vspace_objs_arm_asid_table_unmap:
-  "valid_vspace_objs s
-       \<and> tab = arm_asid_table (arch_state s)
-     \<longrightarrow> valid_vspace_objs (s\<lparr>arch_state := arch_state s\<lparr>arm_asid_table := tab(asid_high_bits_of base := None)\<rparr>\<rparr>)"
-  apply (clarsimp simp: valid_state_def valid_vspace_objs_unmap_strg)
-  done
-
-lemmas arm_context_switch_valid_vspace_objs_aux =
-  hoare_drop_imp[of valid_vspace_objs "arm_context_switch _ _" "\<lambda>_ s. valid_vspace_objs s"
-                , OF arm_context_switch_vspace_objs]
-
-lemma delete_asid_pool_valid_arch_obsj[wp]:
-  "\<lbrace>valid_vspace_objs\<rbrace>
-    delete_asid_pool base pptr
-  \<lbrace>\<lambda>_. valid_vspace_objs\<rbrace>"
-  unfolding delete_asid_pool_def
-  apply (wp modify_wp)
-      apply (strengthen valid_vspace_objs_arm_asid_table_unmap)
-      apply (wpsimp wp: mapM_wp')+
-  done
-
-lemma delete_asid_pool_valid_vspace_objs[wp]:
-  "\<lbrace>valid_vspace_objs\<rbrace>
-    delete_asid_pool base pptr
-  \<lbrace>\<lambda>_. valid_vspace_objs\<rbrace>"
-  unfolding delete_asid_pool_def
-  apply (wp modify_wp)
-      apply (strengthen valid_vspace_objs_arm_asid_table_unmap)
-      apply (wpsimp wp: mapM_wp')+
-  done
-
-crunch valid_vspace_objs[wp]: cap_swap_for_delete "valid_vspace_objs"
-
-lemma set_asid_pool_arch_objs_unmap'':
- "\<lbrace>(valid_vspace_objs and ko_at (ArchObj (ASIDPool ap)) p) and K(f = (ap |` S))\<rbrace> set_asid_pool p f \<lbrace>\<lambda>_. valid_vspace_objs\<rbrace>"
-  apply (rule hoare_gen_asm)
-  apply simp
-  apply (rule set_asid_pool_vspace_objs_unmap)
-  done
-
-lemmas set_asid_pool_vspace_objs_unmap'' = set_asid_pool_arch_objs_unmap''
-
 
 lemma restrict_eq_asn_none: "f(N := None) = f |` {s. s \<noteq> N}" by auto
 
-lemma delete_asid_valid_arch_objs[wp]:
-  "\<lbrace>valid_vspace_objs and pspace_aligned\<rbrace> delete_asid a b \<lbrace>\<lambda>_. valid_vspace_objs\<rbrace>"
-  unfolding delete_asid_def
-  apply (wpsimp wp: set_asid_pool_arch_objs_unmap'')
-  apply (fastforce simp: restrict_eq_asn_none)
-  done
-
-lemma delete_asid_valid_vspace_objs[wp]:
-  "\<lbrace>valid_vspace_objs and pspace_aligned\<rbrace> delete_asid a b \<lbrace>\<lambda>_. valid_vspace_objs\<rbrace>"
-  unfolding delete_asid_def
-  apply (wpsimp wp: set_asid_pool_vspace_objs_unmap'')
-  apply (fastforce simp: restrict_eq_asn_none)
-  done
-
-lemma store_pte_valid_vspace_objs[wp]:
-  "\<lbrace>valid_vspace_objs and valid_pte pte\<rbrace>
-    store_pte p pte
-  \<lbrace>\<lambda>_. (valid_vspace_objs)\<rbrace>"
-  unfolding store_pte_def
-  apply wp
-  apply clarsimp
-  apply (unfold valid_vspace_objs_def)
-  apply (erule_tac x="p && ~~ mask pt_bits" in allE)
-  apply auto
-done
-
-declare get_cap_global_refs[wp]
-
-crunch valid_global_refs[wp]: cap_swap_for_delete "valid_global_refs"
-  (wp: set_cap_globals dxo_wp_weak
-   simp: crunch_simps
-   ignore: set_object cap_swap_ext)
-
-crunch valid_global_refs[wp]: empty_slot "valid_global_refs"
-  (wp: hoare_drop_imps set_cap_globals dxo_wp_weak
-   simp: cap_range_def
-   ignore: set_object empty_slot_ext)
+crunches cap_swap_for_delete
+  for valid_vspace_objs[wp]: valid_vspace_objs
+  and valid_global_refs[wp]: valid_global_refs
+  (simp: crunch_simps)
 
 lemma thread_set_fault_valid_global_refs[wp]:
-  "\<lbrace>valid_global_refs\<rbrace> thread_set (tcb_fault_update A) thread \<lbrace>\<lambda>_. valid_global_refs\<rbrace>"
+  "thread_set (tcb_fault_update A) thread \<lbrace>valid_global_refs\<rbrace>"
   apply (wp thread_set_global_refs_triv thread_set_refs_trivial thread_set_obj_at_impossible | simp)+
   apply (rule ball_tcb_cap_casesI, simp+)
   done
 
-
 lemma cap_swap_for_delete_valid_arch_caps[wp]:
-  "\<lbrace>valid_arch_caps\<rbrace> cap_swap_for_delete a b \<lbrace>\<lambda>_. valid_arch_caps\<rbrace>"
+  "cap_swap_for_delete a b \<lbrace>valid_arch_caps\<rbrace>"
   unfolding cap_swap_for_delete_def
   apply (wp get_cap_wp)
   apply (clarsimp simp: cte_wp_at_weakenE)
   done
 
-lemma mapM_x_swp_store_pte_reads_respects':
-  "reads_respects aag l (invs and (cte_wp_at ((=) (ArchObjectCap (PageTableCap word option))) slot) and K (is_subject aag word))
-                        (mapM_x (swp store_pte InvalidPTE) [word , word + 4 .e. word + 2 ^ pt_bits - 1])"
-  apply (rule gen_asm_ev)
-  apply (wp mapM_x_ev)
-   apply simp
-   apply (rule equiv_valid_guard_imp)
-    apply (wp store_pte_reads_respects)
-   apply simp
-   apply (elim conjE)
-   apply (subgoal_tac "is_aligned word pt_bits")
-    apply (frule (1) word_aligned_pt_slots)
-    apply simp
-   apply (frule cte_wp_valid_cap)
-    apply (rule invs_valid_objs)
-    apply simp
-   apply (simp add: valid_cap_def cap_aligned_def pt_bits_def pageBits_def)
-  apply simp
-  apply wp
-   apply simp
-  apply (fastforce simp: is_cap_simps dest!: cte_wp_at_pt_exists_cap[OF invs_valid_objs])
+(* this to go in InfloFlowBase? *)
+lemma get_object_revrv:
+  "reads_equiv_valid_rv_inv (affects_equiv aag l) aag \<top>\<top> \<top> (get_object ptr)"
+  unfolding get_object_def
+  apply (rule equiv_valid_rv_bind)
+    apply (rule equiv_valid_rv_guard_imp)
+     apply (rule gets_kheap_revrv')
+    apply (simp, simp)
+   apply (rule equiv_valid_2_bind)
+      apply (rule return_ev2)
+      apply (simp)
+     apply (rule assert_ev2)
+     apply (simp)
+    apply (wpsimp)+
   done
 
-lemma mapM_x_swp_store_pde_reads_respects':
-  "reads_respects aag l (cte_wp_at ((=) (ArchObjectCap (PageDirectoryCap word option))) slot and valid_objs and K(is_subject aag word))
-             (mapM_x (swp store_pde InvalidPDE)
-               (map ((\<lambda>x. x + word) \<circ> swp (<<) 2) [0.e.(kernel_base >> 20) - 1]))"
-  apply (wp mapM_x_ev)
-   apply simp
-   apply (rule equiv_valid_guard_imp)
-    apply (wp store_pde_reads_respects)
-   apply clarsimp
-   apply (subgoal_tac "is_aligned word pd_bits")
-    apply (simp add: pd_bits_store_pde_helper)
-   apply (frule (1) cte_wp_valid_cap)
-   apply (simp add: valid_cap_def cap_aligned_def pd_bits_def pageBits_def)
-  apply simp
-  apply wp
-    apply (clarsimp simp: wellformed_pde_def)+
+lemma get_object_revrv':
+  "reads_equiv_valid_rv_inv (affects_equiv aag l) aag
+   (\<lambda>rv rv'. aag_can_read aag ptr \<longrightarrow> rv = rv')
+   \<top> (get_object ptr)"
+  unfolding get_object_def
+  apply (rule equiv_valid_rv_bind)
+    apply (rule equiv_valid_rv_guard_imp)
+     apply (rule gets_kheap_revrv)
+    apply (simp, simp)
+   apply (rule equiv_valid_2_bind)
+      apply (rule return_ev2)
+      apply (simp)
+     apply (rule assert_ev2)
+     apply (simp add: equiv_for_def)
+    apply (wpsimp)+
   done
 
-lemma mapM_x_swp_store_pte_pas_refined_simple:
-  "invariant  (mapM_x (swp store_pte InvalidPTE) A) (pas_refined aag)"
-  by (wpsimp wp: mapM_x_wp' store_pte_pas_refined_simple)
+crunch irq_state_of_state[wp]: cancel_badged_sends "\<lambda>s. P (irq_state_of_state s)"
+  (wp: crunch_wps simp: filterM_mapM)
 
-lemma mapM_x_swp_store_pde_pas_refined_simple:
-  "invariant (mapM_x (swp store_pde InvalidPDE) A) (pas_refined aag)"
-  by (wpsimp wp: mapM_x_wp' store_pde_pas_refined_simple)
+
+locale Arch_IF_1 =
+  fixes valid_ko_at_arch :: "det_state \<Rightarrow> bool"
+  and aag :: "'a PAS"
+  assumes arch_post_cap_deletion_valid_global_refs:
+    "arch_post_cap_deletion acap \<lbrace>\<lambda>s :: det_state. valid_global_refs s\<rbrace>"
+  and arch_post_cap_deletion_irq_state_of_state[wp]:
+    "arch_post_cap_deletion acap \<lbrace>\<lambda>s. P (irq_state_of_state s)\<rbrace>"
+  and store_word_offs_irq_state_of_state[wp]:
+    "store_word_offs ptr offs v \<lbrace>\<lambda>s. P (irq_state_of_state s)\<rbrace>"
+  and set_irq_state_irq_state_of_state[wp]:
+    "set_irq_state state irq \<lbrace>\<lambda>s. P (irq_state_of_state s)\<rbrace>"
+  and handle_arch_fault_reply_irq_state_of_state[wp]:
+    "handle_arch_fault_reply vmf thread x y \<lbrace>\<lambda>s. P (irq_state_of_state s)\<rbrace>"
+  and arch_switch_to_idle_thread_irq_state_of_state[wp]:
+    "arch_switch_to_idle_thread \<lbrace>\<lambda>s. P (irq_state_of_state s)\<rbrace>"
+  and arch_switch_to_thread_irq_state_of_state[wp]:
+    "arch_switch_to_thread t \<lbrace>\<lambda>s. P (irq_state_of_state s)\<rbrace>"
+  and arch_invoke_irq_handler_irq_state_of_state[wp]:
+    "arch_invoke_irq_handler hi \<lbrace>\<lambda>s. P (irq_state_of_state s)\<rbrace>"
+  and arch_finalise_cap_irq_state_of_state[wp]:
+    "arch_finalise_cap acap b \<lbrace>\<lambda>s. P (irq_state_of_state s)\<rbrace>"
+  and prepare_thread_delete_irq_state_of_state[wp]:
+    "prepare_thread_delete t \<lbrace>\<lambda>s. P (irq_state_of_state s)\<rbrace>"
+  and equiv_asid_machine_state_update[simp]:
+    "\<And>f. equiv_asid asid (machine_state_update f s) s' = equiv_asid asid s s'"
+    "\<And>f. equiv_asid asid s (machine_state_update f s') = equiv_asid asid s s'"
+  and as_user_set_register_reads_respects':
+    "pas_domains_distinct aag \<Longrightarrow> reads_respects aag l \<top> (as_user t (setRegister r v))"
+  and store_word_offs_reads_respects:
+    "reads_respects aag l \<top> (store_word_offs ptr offs v)"
+  and set_endpoint_globals_equiv:
+    "\<lbrace>globals_equiv s and valid_ko_at_arch\<rbrace>
+     set_endpoint ptr ep
+     \<lbrace>\<lambda>_. globals_equiv s\<rbrace>"
+  and set_cap_globals_equiv'':
+    "\<lbrace>globals_equiv s and valid_ko_at_arch\<rbrace>
+     set_cap cap p
+     \<lbrace>\<lambda>_. globals_equiv s\<rbrace>"
+  and set_thread_state_globals_equiv:
+    "\<lbrace>globals_equiv s and valid_ko_at_arch\<rbrace>
+     set_thread_state ref ts
+     \<lbrace>\<lambda>_. globals_equiv s\<rbrace>"
+  and as_user_globals_equiv:
+    "\<And>f :: unit user_monad.
+     \<lbrace>globals_equiv s and valid_ko_at_arch and (\<lambda>s. tptr \<noteq> idle_thread s)\<rbrace>
+     as_user tptr f
+     \<lbrace>\<lambda>_. globals_equiv s\<rbrace>"
+  and set_endpoint_valid_ko_at_arch[wp]:
+    "set_endpoint ptr ep \<lbrace>valid_ko_at_arch\<rbrace>"
+  and set_cap_valid_ko_at_arch[wp]:
+    "set_cap cap p \<lbrace>valid_ko_at_arch\<rbrace>"
+  and set_thread_state_valid_ko_at_arch[wp]:
+    "set_thread_state ref ts \<lbrace>valid_ko_at_arch\<rbrace>"
+  and valid_ko_at_arch_exst_update[simp]:
+    "\<And>f. valid_ko_at_arch (trans_state f s) = valid_ko_at_arch s"
+begin
+
+crunch valid_global_refs[wp]: empty_slot "\<lambda>s :: det_state. valid_global_refs s"
+  (simp: cap_range_def)
+
+crunches set_extra_badge, set_mrs, reply_from_kernel, invoke_domain
+  for irq_state_of_state[wp]: "\<lambda>s. P (irq_state_of_state s)"
+  (wp: crunch_wps simp: crunch_simps)
+
+lemma transfer_caps_loop_irq_state[wp]:
+  "transfer_caps_loop a b c d e f \<lbrace>\<lambda>s. P (irq_state_of_state s)\<rbrace>"
+  by (wp transfer_caps_loop_pres)
+
+crunch irq_state_of_state[wp]: handle_recv, handle_reply "\<lambda>s. P (irq_state_of_state s)"
+  (wp: crunch_wps dmo_wp simp: crunch_simps)
+
+crunch irq_state_of_state[wp]: invoke_irq_handler "\<lambda>s. P (irq_state_of_state s)"
+
+crunch irq_state_of_state[wp]: schedule "\<lambda>s. P (irq_state_of_state s)"
+  (wp: dmo_wp modify_wp crunch_wps hoare_whenE_wp
+   simp: machine_op_lift_def machine_rest_lift_def crunch_simps)
+
+crunch irq_state_of_state[wp]: finalise_cap "\<lambda>s. P (irq_state_of_state s)"
+  (wp: select_wp modify_wp crunch_wps dmo_wp simp: crunch_simps)
+
+crunch irq_state_of_state[wp]: send_signal, restart "\<lambda>s. P (irq_state_of_state s)"
+
+lemma mol_states_equiv_for:
+  "machine_op_lift mop \<lbrace>\<lambda>ms. states_equiv_for P Q R S st (s\<lparr>machine_state := ms\<rparr>)\<rbrace>"
+  unfolding machine_op_lift_def
+  apply (simp add: machine_rest_lift_def split_def)
+  apply (wp modify_wp)
+  apply (clarsimp simp: states_equiv_for_def equiv_asids_def)
+  apply (fastforce elim!: equiv_forE intro!: equiv_forI)
+  done
+
+lemma do_machine_op_mol_states_equiv_for:
+  "do_machine_op (machine_op_lift f) \<lbrace>states_equiv_for P Q R S st\<rbrace>"
+  apply (simp add: do_machine_op_def)
+  apply (wp modify_wp | simp add: split_def)+
+  apply (clarify)
+  apply (erule use_valid)
+   apply simp
+   apply (rule mol_states_equiv_for)
+  by simp
+
+lemma set_message_info_reads_respects:
+  assumes domains_distinct: "pas_domains_distinct aag"
+  shows "reads_respects aag l \<top> (set_message_info thread info)"
+  unfolding set_message_info_def fun_app_def
+  by (rule as_user_set_register_reads_respects'[OF domains_distinct])
+
+lemma set_mrs_reads_respects:
+  "reads_respects aag l (K (aag_can_read aag t \<or> aag_can_affect aag l t)) (set_mrs t buf msgs)"
+  apply (simp add: set_mrs_def cong: option.case_cong_weak)
+  apply (wp mapM_x_ev' store_word_offs_reads_respects set_object_reads_respects
+         | wpc | simp add: split_def split del: if_split add: zipWithM_x_mapM_x)+
+  apply (auto intro: reads_affects_equiv_get_tcb_eq)
+  done
+
+crunch valid_ko_at_arch[wp]: set_untyped_cap_as_full valid_ko_at_arch
+
+lemma cap_insert_globals_equiv'':
+  "\<lbrace>globals_equiv s and valid_global_objs and valid_ko_at_arch\<rbrace>
+   cap_insert new_cap src_slot dest_slot
+   \<lbrace>\<lambda>_. globals_equiv s\<rbrace>"
+  unfolding cap_insert_def
+  by (wpsimp wp: set_original_globals_equiv update_cdt_globals_equiv
+                 set_cap_globals_equiv'' dxo_wp_weak hoare_drop_imps)
+
+lemma set_message_info_globals_equiv:
+  "\<lbrace>globals_equiv s and valid_ko_at_arch and (\<lambda>s. thread \<noteq> idle_thread s)\<rbrace>
+   set_message_info thread info
+   \<lbrace>\<lambda>_. globals_equiv s\<rbrace>"
+  unfolding set_message_info_def by (wp as_user_globals_equiv)
+
+lemma cancel_badged_sends_globals_equiv:
+  "\<lbrace>globals_equiv s and valid_ko_at_arch\<rbrace>
+   cancel_badged_sends epptr badge
+   \<lbrace>\<lambda>_. globals_equiv s\<rbrace> "
+  unfolding cancel_badged_sends_def
+  by (wpsimp wp: set_endpoint_globals_equiv set_thread_state_globals_equiv
+                 filterM_preserved dxo_wp_weak hoare_drop_imps)
 
 end
 
